mechanization/theories/Core/Syntactic/System/Definitions.v
@@ -5,6 +5,544 @@ From McPTS.Core Require Import Base.
 From McPTS.Core.Syntactic Require Export Syntax.
 Import Syntax_Notations.
 
+
+Reserved Notation "⊢ Γ" (in custom judg at level 80, Γ custom exp).
+Reserved Notation "⊢ Γ ≈ Γ'" (in custom judg at level 80, Γ custom exp, Γ' custom exp).
+Reserved Notation "Γ ⊢ M : A" (in custom judg at level 80, Γ custom exp, M custom exp, A custom exp).
+Reserved Notation "Γ ⊢ M ≈ M' : A" (in custom judg at level 80, Γ custom exp, M custom exp, M' custom exp, A custom exp).
+Reserved Notation "Γ ⊢ A" (in custom judg at level 80, Γ custom exp, A custom exp).
+Reserved Notation "Γ ⊢ A ≈ A'" (in custom judg at level 80, Γ custom exp, A custom exp, A' custom exp).
+Reserved Notation "Γ ⊢s σ : Δ" (in custom judg at level 80, Γ custom exp, σ custom exp, Δ custom exp).
+Reserved Notation "Γ ⊢s σ ≈ σ' : Δ" (in custom judg at level 80, Γ custom exp, σ custom exp, σ' custom exp, Δ custom exp).
+Reserved Notation "'#' x : A :: K ∈ Γ" (in custom judg at level 80, x constr at level 0, A custom exp, K custom exp, Γ custom exp at level 50).
+
+Generalizable All Variables.
+
+Inductive ctx_lookup {P : PtsSig} : nat -> typ P -> knd P -> ctx P -> Prop :=
+  | here : `({{ #0 : A[Wk] :: K ∈ Γ, A :: K }})
+  | there : `({{ #n : A :: K ∈ Γ }} -> {{ #(S n) : A[Wk] :: K ∈ Γ, B :: L }})
+where "'#' x : A :: K ∈ Γ" := (ctx_lookup x A K Γ) (in custom judg) : type_scope.
+
+Inductive wf_ctx {P : PtsSig} : ctx P -> Prop :=
+| wf_ctx_empty : {{ ⊢ ⋅ }}
+| wf_ctx_extend :
+  `( {{ ⊢ Γ }} ->
+     {{ Γ ⊢ A : Sort@s }} ->
+     {{ ⊢ Γ, A::Sort@s }} )
+where "⊢ Γ" := (wf_ctx Γ) (in custom judg) : type_scope
+
+with wf_exp {P : PtsSig} : ctx P -> typ P -> exp P -> Prop :=
+(** Sorts *)
+| wf_st :
+  `( Ax P s1 s2 -> {{ ⊢ Γ }} ->
+     {{ Γ ⊢ Sort@s1 : Sort@s2 }} )
+
+(** Functions *)
+| wf_pi :
+  `( forall (r : Ru P s1 s2 s3),
+      {{ Γ ⊢ A : Sort@s1 }} ->
+      {{ Γ, A::Sort@s1 ⊢ B : Sort@s2 }} ->
+      {{ Γ ⊢ Π r A B : Sort@s3 }} )
+| wf_fn :
+  `( forall (r : Ru P s1 s2 s3),
+        {{ Γ ⊢ A : Sort@s1 }} ->
+        {{ Γ, A::Sort@s1 ⊢ B : Sort@s2 }} ->
+        {{ Γ, A :: Sort@s1 ⊢ M : B }} ->
+        {{ Γ ⊢ λ r A M : Π r A B }} )
+| wf_app :
+  `( forall (r : Ru P s1 s2 s3),
+        {{ Γ ⊢ A : Sort@s1 }} ->
+        {{ Γ, A::Sort@s1 ⊢ B : Sort@s2 }} ->
+        {{ Γ ⊢ M : Π r A B }} ->
+        {{ Γ ⊢ N : A }} ->
+        {{ Γ ⊢ M N : B[Id,,N] }} )
+
+| wf_vlookup :
+  `( {{ ⊢ Γ }} ->
+     {{ #x : A :: Sort@s ∈ Γ }} ->
+     {{ Γ ⊢ #x : A }} )
+
+
+| wf_exp_sub :
+  `( {{ Γ ⊢s σ : Δ }} ->
+     {{ Δ ⊢ M : A }} ->
+     {{ Γ ⊢ M[σ] : A[σ] }} )
+| wf_exp_conv :
+  `( {{ Γ ⊢ M : A }} ->
+     (** We have this extra argument for soundness.
+         Note that we need to keep it asymmetric:
+         only [A'] is checked. If we check A as well,
+         we cannot even construct something like
+         [{{ Γ ⊢ Type@0[Wk] : Type@1 }}] with the current
+         rules. Under the symmetric rule, the example requires
+         [{{ Γ ⊢ Type@1[Wk] : Type@2 }}] to apply [wf_exp_sub],
+         which requires [{{ Γ ⊢ Type@2[Wk] : Type@3 }}], and so on.
+      *)
+     {{ Γ ⊢ A' }} ->
+     {{ Γ ⊢ A ≈ A' }} ->
+     {{ Γ ⊢ M : A' }} )
+where "Γ ⊢ M : A" := (wf_exp Γ A M) (in custom judg) : type_scope
+
+with wf_typ {P : PtsSig} : ctx P -> typ P -> Prop :=
+| wf_typ_st :
+  `( {{ ⊢ Γ }} ->
+     {{ Γ ⊢ Sort@s }})
+| wf_typ_exp :
+  `( {{ Γ ⊢ A : Sort@s }} ->
+     {{ Γ ⊢ A }})
+| wf_typ_clo :
+  `( {{ Γ ⊢s σ : Δ }} ->
+     {{ Δ ⊢ A }} ->
+     {{ Γ ⊢ A[σ] }})
+where "Γ ⊢ A" := (wf_typ Γ A) (in custom judg) : type_scope
+                                                         
+with wf_sub {P : PtsSig} : ctx P -> ctx P -> sub P -> Prop :=
+| wf_sub_id :
+  `( {{ ⊢ Γ }} ->
+     {{ Γ ⊢s Id : Γ }} )
+| wf_sub_weaken :
+  `( {{ ⊢ Γ, A::Sort@s }} ->
+     {{ Γ, A::Sort@s ⊢s Wk : Γ }} )
+| wf_sub_compose :
+  `( {{ Γ1 ⊢s σ2 : Γ2 }} ->
+     {{ Γ2 ⊢s σ1 : Γ3 }} ->
+     {{ Γ1 ⊢s σ1∘σ2 : Γ3 }} )
+| wf_sub_extend :
+  `( {{ Γ ⊢s σ : Δ }} ->
+     {{ Δ ⊢ A : Sort@s }} ->
+     {{ Γ ⊢ M : A[σ] }} ->
+     {{ Γ ⊢s σ,,M : Δ, A::Sort@s }} )
+| wf_sub_conv :
+  `( {{ Γ ⊢s σ : Δ }} ->
+     (** As in [wf_exp_subtyp], this extra argument is
+         for soundness. We don't need to keep it asymmetric,
+         but do so to match with [wf_exp_subtyp].
+      *)
+     {{ ⊢ Δ' }} ->
+     {{ ⊢ Δ ≈ Δ' }} ->
+     {{ Γ ⊢s σ : Δ' }} )
+where "Γ ⊢s σ : Δ" := (wf_sub Γ Δ σ) (in custom judg) : type_scope
+
+with wf_ctx_eq {P : PtsSig} : ctx P -> ctx P -> Prop :=
+| wf_ctx_eq_empty : {{ ⊢ ⋅ ≈ ⋅ }}
+| wf_ctx_eq_extend :
+  `( {{ ⊢ Γ ≈ Δ }} ->
+     {{ Γ ⊢ A : Sort@s }} ->
+     {{ Γ ⊢ A' : Sort@s }} ->
+     {{ Δ ⊢ A : Sort@s }} ->
+     {{ Δ ⊢ A' : Sort@s }} ->
+     {{ Γ ⊢ A ≈ A' : Sort@s }} ->
+     {{ Δ ⊢ A ≈ A' : Sort@s }} ->
+     {{ ⊢ Γ, A::Sort@s ≈ Δ, A'::Sort@s }} )
+where "⊢ Γ ≈ Γ'" := (wf_ctx_eq Γ Γ') (in custom judg) : type_scope
+                                                          
+with wf_exp_eq {P : PtsSig} : ctx P -> typ P -> exp P -> exp P -> Prop :=
+| wf_exp_eq_typ_sub :
+  `( Ax P s1 s2 ->
+     {{ Γ ⊢s σ : Δ }} ->
+     {{ Γ ⊢ Sort@s1[σ] ≈ Sort@s1 : Sort@s2 }} )
+
+| wf_exp_eq_pi_sub :
+  `( forall (r : Ru P s1 s2 s3),
+        {{ Γ ⊢s σ : Δ }} ->
+        {{ Δ ⊢ A : Sort@s1 }} ->
+        {{ Δ, A::Sort@s1 ⊢ B : Sort@s2 }} ->
+        {{ Γ ⊢ (Π r A B)[σ] ≈ Π r A[σ] B[q σ] : Sort@s3 }} )
+| wf_exp_eq_pi_cong :
+  `( forall (r : Ru P s1 s2 s3),
+        {{ Γ ⊢ A : Sort@s1 }} ->
+        {{ Γ ⊢ A ≈ A' : Sort@s1 }} ->
+        {{ Γ, A::Sort@s1 ⊢ B ≈ B' : Sort@s2 }} ->
+        {{ Γ ⊢ Π r A B ≈ Π r A' B' : Sort@s3 }} )
+| wf_exp_eq_fn_cong :
+  `( forall (r : Ru P s1 s2 s3),
+        {{ Γ ⊢ A : Sort@s1 }} ->
+        {{ Γ ⊢ A ≈ A' : Sort@s1 }} ->
+        {{ Γ, A::Sort@s1 ⊢ B : Sort@s2 }} -> 
+        {{ Γ, A::Sort@s1 ⊢ M ≈ M' : B }} ->
+        {{ Γ ⊢ λ r A M ≈ λ r A' M' : Π r A B }} )
+| wf_exp_eq_fn_sub :
+  `( forall (r : Ru P s1 s2 s3),
+        {{ Γ ⊢s σ : Δ }} ->
+        {{ Δ ⊢ A : Sort@s1 }} ->
+        {{ Δ, A::Sort@s1 ⊢ B : Sort@s2 }} ->
+        {{ Δ, A::Sort@s1 ⊢ M : B }} ->
+        {{ Γ ⊢ (λ r A M)[σ] ≈ λ r A[σ] M[q σ] : (Π r A B)[σ] }} )
+| wf_exp_eq_app_cong :
+  `( forall (r : Ru P s1 s2 s3),
+        {{ Γ ⊢ A : Sort@s1 }} ->
+        {{ Γ, A::Sort@s1 ⊢ B : Sort@s2 }} ->
+        {{ Γ ⊢ M ≈ M' : Π r A B }} ->
+        {{ Γ ⊢ N ≈ N' : A }} ->
+        {{ Γ ⊢ M N ≈ M' N' : B[Id,,N] }} )
+| wf_exp_eq_app_sub :
+  `( forall (r : Ru P s1 s2 s3),
+        {{ Γ ⊢s σ : Δ }} ->
+        {{ Δ ⊢ A : Sort@s1 }} ->
+        {{ Δ, A::Sort@s1 ⊢ B : Sort@s2 }} ->
+        {{ Δ ⊢ M : Π r A B }} ->
+        {{ Δ ⊢ N : A }} ->
+        {{ Γ ⊢ (M N)[σ] ≈ M[σ] N[σ] : B[σ,,N[σ]] }} )
+| wf_exp_eq_pi_beta :
+  `( forall (r : Ru P s1 s2 s3),
+        {{ Γ ⊢ A : Sort@s1 }} ->
+        {{ Γ, A::Sort@s1 ⊢ B : Sort@s2 }} ->
+        {{ Γ, A::Sort@s1 ⊢ M : B }} ->
+        {{ Γ ⊢ N : A }} ->
+        {{ Γ ⊢ (λ r A M) N ≈ M[Id,,N] : B[Id,,N] }} )
+| wf_exp_eq_pi_eta :
+  `( forall (r : Ru P s1 s2 s3),
+        {{ Γ ⊢ A : Sort@s1 }} ->
+        {{ Γ, A::Sort@s1 ⊢ B : Sort@s2 }} ->
+        {{ Γ ⊢ M : Π r A B }} ->
+        {{ Γ ⊢ M ≈ λ r A (M[Wk] #0) : Π r A B }} )
+
+| wf_exp_eq_var :
+  `( {{ ⊢ Γ }} ->
+     {{ #x : A :: Sort@s ∈ Γ }} ->
+     {{ Γ ⊢ #x ≈ #x : A }} )
+| wf_exp_eq_var_0_sub :
+  `( {{ Γ ⊢s σ : Δ }} ->
+     {{ Δ ⊢ A : Sort@s }} ->
+     {{ Γ ⊢ M : A[σ] }} ->
+     {{ Γ ⊢ #0[σ,,M] ≈ M : A[σ] }} )
+| wf_exp_eq_var_S_sub :
+  `( {{ Γ ⊢s σ : Δ }} ->
+     {{ Δ ⊢ A : Sort@s }} ->
+     {{ Γ ⊢ M : A[σ] }} ->
+     {{ #x : B :: Sort@s' ∈ Δ }} ->
+     {{ Γ ⊢ #(S x)[σ,,M] ≈ #x[σ] : B[σ] }} )
+| wf_exp_eq_var_weaken :
+  `( {{ ⊢ Γ, B::Sort@s }} ->
+     {{ #x : A::Sort@s' ∈ Γ }} ->
+     {{ Γ, B::Sort@s ⊢ #x[Wk] ≈ #(S x) : A[Wk] }} )
+| wf_exp_eq_sub_cong :
+  `( {{ Δ ⊢ M ≈ M' : A }} ->
+     {{ Γ ⊢s σ ≈ σ' : Δ }} ->
+     {{ Γ ⊢ M[σ] ≈ M'[σ'] : A[σ] }} )
+| wf_exp_eq_sub_id :
+  `( {{ Γ ⊢ M : A }} ->
+     {{ Γ ⊢ M[Id] ≈ M : A }} )
+| wf_exp_eq_sub_compose :
+  `( {{ Γ ⊢s τ : Γ' }} ->
+     {{ Γ' ⊢s σ : Γ'' }} ->
+     {{ Γ'' ⊢ M : A }} ->
+     {{ Γ ⊢ M[σ∘τ] ≈ M[σ][τ] : A[σ∘τ] }} )
+| wf_exp_eq_conv :
+  `( {{ Γ ⊢ M ≈ M' : A }} ->
+     {{ Γ ⊢ A' }} ->
+     (** This extra argument is here to be consistent with
+         [wf_exp_subtyp].
+      *)
+     {{ Γ ⊢ A ≈ A' }} ->
+     {{ Γ ⊢ M ≈ M' : A' }} )
+| wf_exp_eq_sym :
+  `( {{ Γ ⊢ M ≈ M' : A }} ->
+     {{ Γ ⊢ M' ≈ M : A }} )
+| wf_exp_eq_trans :
+  `( {{ Γ ⊢ M ≈ M' : A }} ->
+     {{ Γ ⊢ M' ≈ M'' : A }} ->
+     {{ Γ ⊢ M ≈ M'' : A }} )
+where "Γ ⊢ M ≈ M' : A" := (wf_exp_eq Γ A M M') (in custom judg) : type_scope
+
+with wf_typ_eq {P : PtsSig} : ctx P -> typ P -> typ P -> Prop :=
+| wf_typ_eq_st :
+  `( {{ ⊢ Γ }} ->
+     {{ Γ ⊢ Sort@s ≈ Sort@s }})
+| wf_typ_eq_sub_st :
+  `( {{ Γ ⊢s σ : Δ }} ->
+     {{ Γ ⊢ Sort@s[σ] ≈ Sort@s}})
+| wf_typ_eq_exp :
+  `( {{ Γ ⊢ A ≈ A' : Sort@s }} ->
+     {{ Γ ⊢ A ≈ A' }})
+| wf_typ_eq_sub_cong :
+  `( {{ Γ ⊢s σ ≈ σ' : Δ }} ->
+     {{ Δ ⊢ A ≈ A' }} ->
+     {{ Γ ⊢ A[σ] ≈ A'[σ'] }})
+| wf_typ_eq_sub_compose :
+  `( {{ Γ ⊢s τ : Γ' }} ->
+     {{ Γ' ⊢s σ : Γ'' }} ->
+     {{ Γ'' ⊢ A }} ->
+     {{ Γ ⊢ A[σ∘τ] ≈ A[σ][τ] }} )
+| wf_typ_eq_sub_id :
+  `( {{ Γ ⊢ A }} ->
+     {{ Γ ⊢ A[Id] ≈ A }} )
+| wf_typ_eq_refl : `({{ Γ ⊢ A }} ->
+                  {{ Γ ⊢ A ≈ A }})
+| wf_typ_eq_sym : `({{ Γ ⊢ A ≈ B }} ->
+                 {{ Γ ⊢ B ≈ A }})
+| wf_typ_eq_trans : `({{ Γ ⊢ A1 ≈ A2 }} -> {{ Γ ⊢ A2 ≈ A3 }} ->
+                   {{ Γ ⊢ A1 ≈ A3 }})
+where "Γ ⊢ A ≈ A'" := (wf_typ_eq Γ A A') (in custom judg) : type_scope
+                                                                    
+with wf_sub_eq {P : PtsSig} : ctx P -> ctx P -> sub P -> sub P -> Prop :=
+| wf_sub_eq_id :
+  `( {{ ⊢ Γ }} ->
+     {{ Γ ⊢s Id ≈ Id : Γ }} )
+| wf_sub_eq_weaken :
+  `( {{ ⊢ Γ, A::Sort@s }} ->
+     {{ Γ, A::Sort@s ⊢s Wk ≈ Wk : Γ }} )
+| wf_sub_eq_compose_cong :
+  `( {{ Γ ⊢s τ ≈ τ' : Γ' }} ->
+     {{ Γ' ⊢s σ ≈ σ' : Γ'' }} ->
+     {{ Γ ⊢s σ∘τ ≈ σ'∘τ' : Γ'' }} )
+| wf_sub_eq_extend_cong :
+  `( {{ Γ ⊢s σ ≈ σ' : Δ }} ->
+     {{ Δ ⊢ A : Sort@s }} ->
+     {{ Γ ⊢ M ≈ M' : A[σ] }} ->
+     {{ Γ ⊢s σ,,M ≈ σ',,M' : Δ, A::Sort@s }} )
+| wf_sub_eq_id_compose_right :
+  `( {{ Γ ⊢s σ : Δ }} ->
+     {{ Γ ⊢s Id∘σ ≈ σ : Δ }} )
+| wf_sub_eq_id_compose_left :
+  `( {{ Γ ⊢s σ : Δ }} ->
+     {{ Γ ⊢s σ∘Id ≈ σ : Δ }} )
+| wf_sub_eq_compose_assoc :
+  `( {{ Γ' ⊢s σ : Γ }} ->
+     {{ Γ'' ⊢s σ' : Γ' }} ->
+     {{ Γ''' ⊢s σ'' : Γ'' }} ->
+     {{ Γ''' ⊢s (σ∘σ')∘σ'' ≈ σ∘(σ'∘σ'') : Γ }} )
+| wf_sub_eq_extend_compose :
+  `( {{ Γ' ⊢s σ : Γ'' }} ->
+     {{ Γ'' ⊢ A : Sort@s }} ->
+     {{ Γ' ⊢ M : A[σ] }} ->
+     {{ Γ ⊢s τ : Γ' }} ->
+     {{ Γ ⊢s (σ,,M)∘τ ≈ (σ∘τ),,M[τ] : Γ'', A::Sort@s }} )
+| wf_sub_eq_p_extend :
+  `( {{ Γ' ⊢s σ : Γ }} ->
+     {{ Γ ⊢ A : Sort@s }} ->
+     {{ Γ' ⊢ M : A[σ] }} ->
+     {{ Γ' ⊢s Wk∘(σ,,M) ≈ σ : Γ }} )
+| wf_sub_eq_extend :
+  `( {{ Γ' ⊢s σ : Γ, A::Sort@s }} ->
+     {{ Γ' ⊢s σ ≈ (Wk∘σ),,#0[σ] : Γ, A::Sort@s }} )
+| wf_sub_eq_sym :
+  `( {{ Γ ⊢s σ ≈ σ' : Δ }} ->
+     {{ Γ ⊢s σ' ≈ σ : Δ }} )
+| wf_sub_eq_trans :
+  `( {{ Γ ⊢s σ ≈ σ' : Δ }} ->
+     {{ Γ ⊢s σ' ≈ σ'' : Δ }} ->
+     {{ Γ ⊢s σ ≈ σ'' : Δ }} )
+| wf_sub_eq_conv :
+  `( {{ Γ ⊢s σ ≈ σ' : Δ }} ->
+     (** This extra argument is here to be consistent with
+         [wf_sub_subtyp].
+      *)
+     {{ ⊢ Δ' }} ->
+     {{ ⊢ Δ ≈ Δ' }} ->
+     {{ Γ ⊢s σ ≈ σ' : Δ' }} )
+where "Γ ⊢s σ ≈ σ' : Δ" := (wf_sub_eq Γ Δ σ σ') (in custom judg) : type_scope.
+
+Scheme wf_ctx_mut_ind := Induction for wf_ctx Sort Prop
+with wf_ctx_eq_mut_ind := Induction for wf_ctx_eq Sort Prop
+with wf_exp_mut_ind := Induction for wf_exp Sort Prop
+with wf_exp_eq_mut_ind := Induction for wf_exp_eq Sort Prop
+with wf_typ_mut_ind := Induction for wf_typ Sort Prop
+with wf_typ_eq_mut_ind := Induction for wf_typ_eq Sort Prop
+with wf_sub_mut_ind := Induction for wf_sub Sort Prop
+with wf_sub_eq_mut_ind := Induction for wf_sub_eq Sort Prop.
+Combined Scheme syntactic_wf_mut_ind from
+  wf_ctx_mut_ind,
+  wf_ctx_eq_mut_ind,
+  wf_exp_mut_ind,
+  wf_exp_eq_mut_ind,
+  wf_typ_mut_ind,
+  wf_typ_eq_mut_ind,
+  wf_sub_mut_ind,
+  wf_sub_eq_mut_ind.
+
+Scheme wf_ctx_mut_ind' := Induction for wf_ctx Sort Prop
+with wf_exp_mut_ind' := Induction for wf_exp Sort Prop
+with wf_typ_eq_mut_ind' := Induction for wf_typ_eq Sort Prop.
+Combined Scheme syntactic_wf_mut_ind' from
+  wf_ctx_mut_ind',
+  wf_exp_mut_ind',
+  wf_typ_eq_mut_ind'.
+
+
+#[export]
+Hint Constructors wf_ctx wf_ctx_eq wf_exp wf_typ wf_sub wf_exp_eq wf_typ_eq wf_sub_eq ctx_lookup : mcpts.
+
+#[export]
+Instance wf_exp_eq_PER {P : PtsSig} (Γ : ctx P) A : PER (wf_exp_eq Γ A).
+Proof.
+  split.
+  - eauto using wf_exp_eq_sym.
+  - eauto using wf_exp_eq_trans.
+Qed.
+
+#[export]
+Instance wf_typ_eq_PER {P : PtsSig} (Γ : ctx P) : PER (wf_typ_eq Γ).
+Proof.
+  split.
+  - eauto using wf_typ_eq_sym.
+  - eauto using wf_typ_eq_trans.
+Qed.
+
+#[export]
+Instance wf_sub_eq_PER {P : PtsSig} (Γ : ctx P) Δ : PER (wf_sub_eq Γ Δ).
+Proof.
+  split.
+  - eauto using wf_sub_eq_sym.
+  - eauto using wf_sub_eq_trans.
+Qed.
+
+
+
+Instance wf_ctx_eq_Symmetric {P : PtsSig} : Symmetric (@wf_ctx_eq P).
+Proof.
+  induction 1; mauto.
+Qed.
+
+(** Immediate & Independent Presuppositions *)
+
+Lemma presup_wf_ctx_eq {P : PtsSig} : forall {Γ Δ : ctx P}, {{ ⊢ Γ ≈ Δ }} -> {{ ⊢ Γ }} /\ {{ ⊢ Δ }}.
+Proof with mautosolve.
+  induction 1; destruct_pairs...
+Qed.
+
+#[export]
+Hint Resolve presup_wf_ctx_eq : mcpts.
+
+Lemma presup_wf_ctx_eq_left {P : PtsSig} : forall {Γ Δ : ctx P}, {{ ⊢ Γ ≈ Δ }} -> {{ ⊢ Γ }}.
+Proof with easy.
+  intros * ?%presup_wf_ctx_eq...
+Qed.
+
+#[export]
+Hint Resolve presup_wf_ctx_eq_left : mcpts.
+
+Lemma presup_wf_ctx_eq_right {P : PtsSig} : forall {Γ Δ : ctx P}, {{ ⊢ Γ ≈ Δ }} -> {{ ⊢ Δ }}.
+Proof with easy.
+  intros * ?%presup_wf_ctx_eq...
+Qed.
+
+#[export]
+Hint Resolve presup_wf_ctx_eq_right : mcpts.
+
+(* All of the following lemmas about subtyping should be replaced with lemmas about type equality 
+ * But this essentially means proving the whole presupposition lemma, so we will do it later intead
+ *)
+(* Lemma presup_subtyp_right : forall {Γ A B}, {{ Γ ⊢ A ⊆ B }} -> exists i, {{ Γ ⊢ B : Type@i }}. *)
+(* Proof with mautosolve. *)
+(*   induction 1... *)
+(* Qed. *)
+
+(* #[export] *)
+(* Hint Resolve presup_subtyp_right : mcpts. *)
+
+(* (** Subtyping Rules without Extra Arguments *) *)
+
+(* Lemma wf_exp_subtyp' : forall Γ A A' M, *)
+(*     {{ Γ ⊢ M : A }} -> *)
+(*     {{ Γ ⊢ A ⊆ A' }} -> *)
+(*     {{ Γ ⊢ M : A' }}. *)
+(* Proof. *)
+(*   intros. *)
+(*   assert (exists i, {{ Γ ⊢ A' : Type@i }}) as [] by mauto. *)
+(*   econstructor; mauto. *)
+(* Qed. *)
+
+(* #[export] *)
+(* Hint Resolve wf_exp_subtyp' : mcpts. *)
+(* #[export] *)
+(* Remove Hints wf_exp_subtyp : mcpts. *)
+
+(* Lemma wf_sub_subtyp' : forall Γ Δ Δ' σ, *)
+(*     {{ Γ ⊢s σ : Δ }} -> *)
+(*     {{ ⊢ Δ ⊆ Δ' }} -> *)
+(*     {{ Γ ⊢s σ : Δ' }}. *)
+(* Proof. *)
+(*   intros. *)
+(*   econstructor; mauto. *)
+(* Qed. *)
+
+(* #[export] *)
+(* Hint Resolve wf_sub_subtyp' : mcpts. *)
+(* #[export] *)
+(* Remove Hints wf_sub_subtyp : mcpts. *)
+
+(* Lemma wf_exp_eq_subtyp' : forall Γ A A' M M', *)
+(*     {{ Γ ⊢ M ≈ M' : A }} -> *)
+(*     {{ Γ ⊢ A ⊆ A' }} -> *)
+(*     {{ Γ ⊢ M ≈ M' : A' }}. *)
+(* Proof. *)
+(*   intros. *)
+(*   assert (exists i, {{ Γ ⊢ A' : Type@i }}) as [] by mauto. *)
+(*   econstructor; mauto. *)
+(* Qed. *)
+
+(* #[export] *)
+(* Hint Resolve wf_exp_eq_subtyp' : mcpts. *)
+(* #[export] *)
+(* Remove Hints wf_exp_eq_subtyp : mcpts. *)
+
+(* Lemma wf_sub_eq_subtyp' : forall Γ Δ Δ' σ σ', *)
+(*     {{ Γ ⊢s σ ≈ σ' : Δ }} -> *)
+(*     {{ ⊢ Δ ⊆ Δ' }} -> *)
+(*     {{ Γ ⊢s σ ≈ σ' : Δ' }}. *)
+(* Proof. *)
+(*   intros. *)
+(*   econstructor; mauto. *)
+(* Qed. *)
+
+(* #[export] *)
+(* Hint Resolve wf_sub_eq_subtyp' : mcpts. *)
+(* #[export] *)
+(* Remove Hints wf_sub_eq_subtyp : mcpts. *)
+
+Add Parametric Morphism {P : PtsSig} (Γ : ctx P) T : (wf_exp_eq Γ T)
+    with signature wf_exp_eq Γ T ==> eq ==> iff as wf_exp_eq_morphism_iff1.
+Proof.
+  split; mauto.
+Qed.
+
+Add Parametric Morphism {P : PtsSig} (Γ : ctx P) T : (wf_exp_eq Γ T)
+    with signature eq ==> wf_exp_eq Γ T ==> iff as wf_exp_eq_morphism_iff2.
+Proof.
+  split; mauto.
+Qed.
+
+Add Parametric Morphism {P : PtsSig} (Γ : ctx P) Δ : (wf_sub_eq Γ Δ)
+    with signature wf_sub_eq Γ Δ ==> eq ==> iff as wf_sub_eq_morphism_iff1.
+Proof.
+  split; mauto.
+Qed.
+
+Add Parametric Morphism {P : PtsSig} (Γ : ctx P) Δ : (wf_sub_eq Γ Δ)
+    with signature eq ==> wf_sub_eq Γ Δ ==> iff as wf_sub_eq_morphism_iff2.
+Proof.
+  split; mauto.
+Qed.
+
+#[export]
+Hint Rewrite -> @wf_exp_eq_typ_sub using mauto 3 : mcpts.
+
+#[export]
+Hint Rewrite -> @wf_sub_eq_id_compose_right @wf_sub_eq_id_compose_left
+                  @wf_sub_eq_compose_assoc (* prefer right association *)
+                  @wf_sub_eq_p_extend using mauto 4 : mcpts.
+
+#[export]
+Hint Rewrite -> @wf_exp_eq_sub_id @wf_exp_eq_pi_sub using mauto 4 : mcpts.
+
+#[export]
+Instance wf_exp_eq_per_elem {P : PtsSig} (Γ : ctx P) T : PERElem _ (wf_exp Γ T) (wf_exp_eq Γ T).
+Proof.
+  intros a Ha. mauto.
+Qed.
+
+
+#[export]
+Instance wf_sub_eq_per_elem {P : PtsSig} (Γ : ctx P) Δ : PERElem _ (wf_sub Γ Δ) (wf_sub_eq Γ Δ).
+Proof.
+  intros a Ha. mauto.
+Qed.
+
+
+
+
+(*
 Reserved Notation "⊢ Γ" (in custom judg at level 80, Γ custom Exp).
 Reserved Notation "⊢ Γ ≈ Δ" (in custom judg at level 80, Γ custom Exp, Δ custom Exp).
 Reserved Notation "Γ ⊢ M : A" (in custom judg at level 80, Γ custom Exp, M custom Exp, A custom Exp).
@@ -313,3 +851,5 @@ Instance wf_sub_eq_per_elem {P : PtsSig} (Γ Δ : Ctx P) : PERElem _ (wf_sub Γ 
 Proof.
   intros a Ha; econstructor; mauto.
 Qed.
+
+*)
