mechanization/theories/Core/Syntactic/CoreInversions.v
@@ -4,7 +4,179 @@ From McPTS.Core Require Import Base.
 From McPTS.Core.Syntactic Require Export CtxEq.
 Import Syntax_Notations.
 
-Lemma wf_pi_inversion {P : PtsSig} : forall {Γ : Ctx P} {A B C s1 s2 s3} {r : Ru P s1 s2 s3},
+
+Lemma wf_pi_inversion {P : PtsSig} : forall {Γ : ctx P} {A B C s1 s2 s3} {r : Ru P s1 s2 s3},
+    {{ Γ ⊢ Π r A B : C }} ->
+    {{ Γ ⊢ A : Sort@s1 }} /\ {{ Γ, A::Sort@s1 ⊢ B : Sort@s2 }} /\ {{ Γ ⊢ Sort@s3 ≈ C }}.
+Proof with mautosolve 4.  
+  intros * H.
+  dependent induction H;
+    gen_core_presups; mauto.
+  split; [|split];
+    [| | transitivity A0; mauto 2];
+    eapply IHwf_exp; mauto 2.
+Qed.
+
+#[export]
+Hint Resolve wf_pi_inversion : mcpts.
+
+(* I am not sure this is really relevant in our setting *)
+Corollary wf_pi_inversion' {P : PtsSig} : forall {Γ : ctx P} {A B C s1 s2 s3} {r : Ru P s1 s2 s3},
+    {{ Γ ⊢ Π r A B : C }} ->
+    {{ Γ ⊢ A : Sort@s1 }} /\ {{ Γ, A::Sort@s1 ⊢ B : Sort@s2 }}.
+Proof with mautosolve 4.
+  intros.
+  assert ({{ Γ ⊢ A : Sort@s1 }} /\ {{ Γ, A::Sort@s1 ⊢ B : Sort@s2 }} /\ {{ Γ ⊢ Sort@s3 ≈ C }}) by (eapply wf_pi_inversion; mauto 2).
+  destruct_conjs; mauto 2.
+Qed.
+
+#[export]
+Hint Resolve wf_pi_inversion' : mcpts.
+
+Corollary wf_typ_pi_inversion {P : PtsSig} : forall {Γ : ctx P} {A B s1 s2 s3} {r : Ru P s1 s2 s3},
+    {{ Γ ⊢ Π r A B }} ->
+    {{ Γ ⊢ A : Sort@s1 }} /\ {{ Γ, A::Sort@s1 ⊢ B : Sort@s2 }}.
+Proof.
+  intros * H; inversion H; mauto 2.
+Qed.
+
+#[export]
+Hint Resolve wf_typ_pi_inversion : mcpts.
+
+Corollary wf_fn_inversion {P : PtsSig} : forall {Γ : ctx P} {A M C s1 s2 s3} {r : Ru P s1 s2 s3},
+    {{ Γ ⊢ λ r A M : C }} ->
+    exists B, {{ Γ, A::Sort@s1 ⊢ M : B }} /\ {{ Γ ⊢ Π r A B ≈ C }}.
+Proof with solve [mauto].
+  intros * H.
+  dependent induction H;
+    gen_core_presups.
+  - eexists; split; mauto.
+  - assert (exists B, {{ Γ, A::Sort@s1 ⊢ M : B }} /\ {{ Γ ⊢ Π r A B ≈ A0 }}) by (eapply IHwf_exp; mauto).
+  destruct_conjs.
+  eexists; split; mauto.
+Qed.
+
+#[export]
+Hint Resolve wf_fn_inversion : mcpts.
+
+Lemma wf_app_inversion {P : PtsSig} : forall {Γ : ctx P} {M N C},
+    {{ Γ ⊢ M N : C }} ->
+    exists A B s1 s2 s3 (r : Ru P s1 s2 s3), {{ Γ ⊢ M : Π r A B }} /\ {{ Γ ⊢ N : A }} /\ {{ Γ ⊢ B[Id,,N] ≈ C }}.
+Proof with mautosolve 4.
+  intros * H.
+  dependent induction H;
+    gen_core_presups.
+  - do 6 eexists; repeat split; eauto.
+    eapply wf_typ_eq_refl.
+    assert {{ Γ ⊢ Π r A B : Sort@s3 }} by mauto.
+    assert ({{ Γ ⊢ A : Sort@s1 }} /\ {{ Γ, A::Sort@s1 ⊢ B : Sort@s2 }}) by mauto.
+    destruct_conjs.
+    econstructor; mauto 3.
+  - assert (exists A0 B s1 s2 s3 r, {{ Γ ⊢ M : Π r A0 B }} /\ {{ Γ ⊢ N : A0 }} /\ {{ Γ ⊢ B[Id,,N] ≈ A }}) by (eapply IHwf_exp; mauto).
+    destruct_conjs.
+    do 6 eexists; repeat split; mauto.  
+Qed.
+
+#[export]
+Hint Resolve wf_app_inversion : mcpts.
+
+Lemma wf_vlookup_inversion {P : PtsSig} : forall {Γ : ctx P} {x A},
+    {{ Γ ⊢ #x : A }} ->
+    exists A' K, {{ #x : A' :: K ∈ Γ }} /\ {{ Γ ⊢ A' ≈ A }}.
+Proof with mautosolve 4.
+  intros * H.
+  dependent induction H;
+    gen_core_presups.
+  - do 2 eexists; split; mauto.
+  - assert (exists A' K, {{ #x : A' :: K ∈ Γ }} /\ {{ Γ ⊢ A' ≈ A0 }}) by (eapply IHwf_exp; mauto).
+    destruct_conjs.
+    do 2 eexists; split; mauto.
+Qed.
+
+#[export]
+Hint Resolve wf_vlookup_inversion : mcpts.
+
+Lemma wf_exp_sub_inversion {P : PtsSig} : forall {Γ : ctx P} {M σ A},
+    {{ Γ ⊢ M[σ] : A }} ->
+    exists Δ A', {{ Γ ⊢s σ : Δ }} /\ {{ Δ ⊢ M : A' }} /\ {{ Γ ⊢ A'[σ] ≈ A }}.
+Proof with mautosolve 3.
+  intros * H.
+  dependent induction H;
+    gen_core_presups.
+  - do 2 eexists; repeat split; mauto.
+  - assert (exists Δ A', {{ Γ ⊢s σ : Δ }} /\ {{ Δ ⊢ M : A' }} /\ {{ Γ ⊢ A'[σ] ≈ A0 }}) by (eapply IHwf_exp; mauto).
+    destruct_conjs.
+    do 2 eexists; repeat split; mauto.  
+Qed.
+
+#[export]
+Hint Resolve wf_exp_sub_inversion : mcpts.
+
+(** We omit [wf_conv] and [wf_cumu] as they do not give useful inversions *)
+
+Lemma wf_sub_id_inversion {P : PtsSig} : forall (Γ : ctx P) Δ,
+    {{ Γ ⊢s Id : Δ }} ->
+    {{ ⊢ Γ ≈ Δ }}.
+Proof.
+  intros * H.
+  dependent induction H; mautosolve 3.
+Qed.
+
+#[export]
+Hint Resolve wf_sub_id_inversion : mcpts.
+
+Lemma wf_sub_weaken_inversion {P : PtsSig} : forall {Γ : ctx P} {Δ},
+    {{ Γ ⊢s Wk : Δ }} ->
+    exists Γ' A s, {{ ⊢ Γ ≈ Γ', A::Sort@s }} /\ {{ ⊢ Γ' ≈ Δ }}.
+Proof.
+  intros * H.
+  
+  dependent induction H;
+    firstorder;
+    progressive_inversion.  
+  - repeat eexists; mauto 2.
+  - assert (exists Γ' A s, {{ ⊢ Γ ≈ Γ', A::Sort@s }} /\ {{ ⊢ Γ' ≈ Δ0 }}) by (eapply IHwf_sub; mauto).
+    destruct_conjs.
+    repeat eexists; mauto 2.
+Qed.
+
+#[export]
+Hint Resolve wf_sub_weaken_inversion : mcpts.
+
+Lemma wf_sub_compose_inversion {P : PtsSig} : forall {Γ1 : ctx P} {σ1 σ2 Γ3},
+    {{ Γ1 ⊢s σ1 ∘ σ2 : Γ3 }} ->
+    exists Γ2, {{ Γ1 ⊢s σ2 : Γ2 }} /\ {{ Γ2 ⊢s σ1 : Γ3 }}.
+Proof with mautosolve 3.
+  intros * H.
+  dependent induction H; mauto 3.
+  assert (exists Γ2, {{ Γ ⊢s σ2 : Γ2 }} /\ {{ Γ2 ⊢s σ1 : Δ }}) by (eapply IHwf_sub; mauto).
+  destruct_conjs.
+  eexists; split; mauto.
+Qed.
+
+#[export]
+Hint Resolve wf_sub_compose_inversion : mcpts.
+
+Lemma wf_sub_extend_inversion {P : PtsSig} : forall {Γ : ctx P} {σ M Δ},
+    {{ Γ ⊢s σ,,M : Δ }} ->
+    exists Δ' A' s', {{ ⊢ Δ', A'::Sort@s' ≈ Δ }} /\ {{ Γ ⊢s σ : Δ' }} /\ {{ Γ ⊢ M : A'[σ] }}.
+Proof with mautosolve 4.
+  intros * H.
+  dependent induction H;
+    gen_core_presups.
+  - repeat eexists...
+  - assert (exists Δ' A' s', {{ ⊢ Δ', A'::Sort@s' ≈ Δ0 }} /\ {{ Γ ⊢s σ : Δ' }} /\ {{ Γ ⊢ M : A'[σ] }}) by (eapply IHwf_sub; mauto).
+    destruct_conjs.
+    repeat eexists...
+Qed.
+
+#[export]
+Hint Resolve wf_sub_extend_inversion : mcpts.
+
+
+
+(*
+Lemma wf_pi_inversion {P : PtsSig} : forall {Γ : ctx P} {A B C s1 s2 s3} {r : Ru P s1 s2 s3},
     {{ Γ ⊢ Π r A B : C }} ->
     {{ Γ ⊢ A : Sort@s1 }} /\ {{ Γ, A::Sort@s1 ⊢ B : Sort@s2 }} /\ {{ Γ ⊢ Sort@s3 ≈ C }}.
 Proof with mautosolve 4.
@@ -22,7 +194,7 @@ Qed.
 #[export]
 Hint Resolve wf_pi_inversion : mcpts.
 
-Corollary wf_pi_inversion' {P : PtsSig} : forall {Γ : Ctx P} {A B s1 s2 s3} {r : Ru P s1 s2 s3},
+Corollary wf_pi_inversion' {P : PtsSig} : forall {Γ : ctx P} {A B s1 s2 s3} {r : Ru P s1 s2 s3},
     {{ Γ ⊢ Π r A B : Sort@s3 }} ->
     {{ Γ ⊢ A : Sort@s1 }} /\ {{ Γ, A::Sort@s1 ⊢ B : Sort@s2 }}.
 Proof with mautosolve 4.
@@ -32,7 +204,7 @@ Proof with mautosolve 4.
   split; assumption.
 Qed.
 
-Corollary wf_typ_pi_inversion {P : PtsSig} : forall {Γ : Ctx P} {A B s1 s2 s3} {r : Ru P s1 s2 s3},
+Corollary wf_typ_pi_inversion {P : PtsSig} : forall {Γ : ctx P} {A B s1 s2 s3} {r : Ru P s1 s2 s3},
     {{ Γ ⊢ Π r A B }} ->
     {{ Γ ⊢ Π r A B : Sort@s3 }}.
 Proof.
@@ -47,7 +219,7 @@ Qed.
 #[export]
 Hint Resolve wf_pi_inversion' wf_typ_pi_inversion : mcpts.
 
-Corollary wf_fn_inversion {P : PtsSig} : forall {Γ : Ctx P} {A M C s1 s2 s3} {r : Ru P s1 s2 s3},
+Corollary wf_fn_inversion {P : PtsSig} : forall {Γ : ctx P} {A M C s1 s2 s3} {r : Ru P s1 s2 s3},
     {{ Γ ⊢ λ r A M : C }} ->
     exists B, {{ Γ, A::Sort@s1 ⊢ M : B }} /\ {{ Γ ⊢ Π r A B ≈ C }}.
 Proof with solve [mauto].
@@ -69,33 +241,28 @@ Qed.
 #[export]
 Hint Resolve wf_fn_inversion : mcpts.
 
-Lemma wf_app_inversion {P : PtsSig} : forall {Γ : Ctx P} {M N C},
+Lemma wf_app_inversion {P : PtsSig} : forall {Γ : ctx P} {M N C},
     {{ Γ ⊢ M N : C }} ->
-    exists A B s1 s2 s3 (r : Ru P s1 s2 s3), {{ Γ ⊢ M : Π r A B }} /\ {{ Γ ⊢ N : A }} /\ {{ Γ ⊢ [Id,,N]B ≈ C }}.
+    exists A B s1 s2 s3 (r : Ru P s1 s2 s3), {{ Γ ⊢ M : Π r A B }} /\ {{ Γ ⊢ N : A }} /\ {{ Γ ⊢ B[Id,,N] ≈ C }}.
 Proof with mautosolve 4.
   intros * H.
   dependent induction H.
   - destruct_conjs; 
       do 6 eexists; repeat split; eauto.
     (* reflexivity. *)
-    eapply eq_typ_refl.
+    eapply wf_typ_eq_refl.
     assert {{ Γ ⊢ Π r A B : Sort@s3 }} by mauto.
-    assert ({{ Γ ⊢ A : Sort@s1 }} /\ {{ Γ, A::Sort@s1 ⊢ B : Sort@s2 }}).
-    {
-      eapply wf_pi_inversion'; mauto 2.
-    }
+    assert ({{ Γ ⊢ A : Sort@s1 }} /\ {{ Γ, A::Sort@s1 ⊢ B : Sort@s2 }}) by mauto.
     destruct_conjs.
-    econstructor; mauto 2.
-  - specialize (IHwf_exp _ _ eq_refl); 
-      destruct_conjs;
-      do 6 eexists; repeat split; eauto.
-    transitivity {{{ A }}}; mauto 2.
-Qed.
+    econstructor; mauto 3.
+  - eapply IHwf_exp; try reflexivity.    
+    admit. (* I don't even know what this goal means *)
+Admitted.
 
 #[export]
 Hint Resolve wf_app_inversion : mcpts.
 
-Lemma wf_vlookup_inversion {P : PtsSig} : forall {Γ : Ctx P} {x A},
+Lemma wf_vlookup_inversion {P : PtsSig} : forall {Γ : ctx P} {x A},
     {{ Γ ⊢ #x : A }} ->
     exists A' s, {{ #x : A' :: Sort@s ∈ Γ }} /\ {{ Γ ⊢ A' ≈ A }}.
 Proof with mautosolve 4.
@@ -103,21 +270,20 @@ Proof with mautosolve 4.
   dependent induction H.
   - exists A; exists s.
     split; mauto 2.
-    eapply eq_typ_refl.
+    eapply wf_typ_eq_refl.
     econstructor; mauto 2.
-  - specialize (IHwf_exp _ eq_refl).
-    destruct IHwf_exp as [A' HA'].
-    destruct HA' as [s [HA'1 HA'2]].
-    exists A'; exists s.
-    split; mauto 2.
-Qed.
+    eapply presup_ctx_lookup_typ; mauto.
+    
+  - eapply IHwf_exp; mauto.
+    admit. (* Again with the weird the goal *)
+Admitted.
 
 #[export]
 Hint Resolve wf_vlookup_inversion : mcpts.
 
-Lemma wf_exp_sub_inversion {P : PtsSig} : forall {Γ : Ctx P} {M σ A},
-    {{ Γ ⊢ [σ]M : A }} ->
-    exists Δ A', {{ Γ ⊢s σ : Δ }} /\ {{ Δ ⊢ M : A' }} /\ {{ Γ ⊢ [σ]A' ≈ A }}.
+Lemma wf_exp_sub_inversion {P : PtsSig} : forall {Γ : ctx P} {M σ A},
+    {{ Γ ⊢ M[σ] : A }} ->
+    exists Δ A', {{ Γ ⊢s σ : Δ }} /\ {{ Δ ⊢ M : A' }} /\ {{ Γ ⊢ A'[σ] ≈ A }}.
 Proof with mautosolve 3.
   intros * H.
   dependent induction H.
@@ -139,7 +305,7 @@ Hint Resolve wf_exp_sub_inversion : mcpts.
 
 (** We omit [wf_conv] and [wf_cumu] as they do not give useful inversions *)
 
-Lemma wf_sub_id_inversion {P : PtsSig} : forall (Γ Δ : Ctx P),
+Lemma wf_sub_id_inversion {P : PtsSig} : forall (Γ Δ : ctx P),
     {{ Γ ⊢s Id : Δ }} ->
     {{ ⊢ Γ ≈ Δ }}.
 Proof.
@@ -150,7 +316,7 @@ Qed.
 #[export]
 Hint Resolve wf_sub_id_inversion : mcpts.
 
-Lemma wf_sub_weaken_inversion {P : PtsSig} : forall {Γ Δ : Ctx P},
+Lemma wf_sub_weaken_inversion {P : PtsSig} : forall {Γ Δ : ctx P},
     {{ Γ ⊢s Wk : Δ }} ->
     exists Γ' A s, {{ ⊢ Γ ≈ Γ', A::Sort@s }} /\ {{ ⊢ Γ' ≈ Δ }}.
 Proof.
@@ -164,7 +330,7 @@ Qed.
 #[export]
 Hint Resolve wf_sub_weaken_inversion : mcpts.
 
-Lemma wf_sub_compose_inversion {P : PtsSig} : forall {Γ1 : Ctx P} {σ1 σ2 Γ3},
+Lemma wf_sub_compose_inversion {P : PtsSig} : forall {Γ1 : ctx P} {σ1 σ2 Γ3},
     {{ Γ1 ⊢s σ2 ∘ σ1 : Γ3 }} ->
     exists Γ2, {{ Γ1 ⊢s σ2 : Γ2 }} /\ {{ Γ2 ⊢s σ1 : Γ3 }}.
 Proof with mautosolve 3.
@@ -179,7 +345,7 @@ Qed.
 #[export]
 Hint Resolve wf_sub_compose_inversion : mcpts.
 
-Lemma wf_sub_extend_inversion {P : PtsSig} : forall {Γ : Ctx P} {σ M Δ},
+Lemma wf_sub_extend_inversion {P : PtsSig} : forall {Γ : ctx P} {σ M Δ},
     {{ Γ ⊢s σ,,M : Δ }} ->
     exists Δ' A' s, {{ ⊢ Δ', A'::Sort@s ≈ Δ }} /\ {{ Γ ⊢s σ : Δ' }} /\ {{ Γ ⊢ M : [σ]A' }}.
 Proof with mautosolve 4.
@@ -192,3 +358,5 @@ Qed.
 
 #[export]
 Hint Resolve wf_sub_extend_inversion : mcpts.
+
+*)
