mechanization/theories/Core/Syntactic/CtxEq.v
@@ -3,16 +3,16 @@ From McPTS.Core Require Import Base.
 From McPTS.Core.Syntactic Require Export System.
 Import Syntax_Notations.
 
-Lemma ctx_eq_refl {P : PtsSig} : forall {Γ : Ctx P}, {{ ⊢ Γ }} -> {{ ⊢ Γ ≈ Γ }}.
+
+Lemma ctx_eq_refl {P : PtsSig} : forall {Γ : ctx P}, {{ ⊢ Γ }} -> {{ ⊢ Γ ≈ Γ }}.
 Proof with mautosolve.
-  intros *.
-  induction 1; econstructor; mauto 2; econstructor; mauto 2.
+  induction 1...
 Qed.
 
 #[export]
 Hint Resolve ctx_eq_refl : mcpts.
 
-Lemma ctx_eq_sym {P : PtsSig} : forall {Γ Δ : Ctx P}, {{ ⊢ Γ ≈ Δ }} -> {{ ⊢ Δ ≈ Γ }}.
+Lemma ctx_eq_sym {P : PtsSig} : forall {Γ Δ : ctx P}, {{ ⊢ Γ ≈ Δ }} -> {{ ⊢ Δ ≈ Γ }}.
 Proof.
   intros.
   symmetry.
@@ -35,17 +35,17 @@ match type of H with
 end.
 
 #[local]
-Lemma ctxeq_exp_helper {P : PtsSig} : forall {Γ : Ctx P} {M A}, {{ Γ ⊢ M : A }} -> forall {Δ}, {{ ⊢ Δ ≈ Γ }} -> {{ Δ ⊢ M : A }}
+Lemma ctxeq_exp_helper {P : PtsSig} : forall {Γ : ctx P} {M A}, {{ Γ ⊢ M : A }} -> forall {Δ}, {{ ⊢ Δ ≈ Γ }} -> {{ Δ ⊢ M : A }}
 with
-ctxeq_exp_eq_helper {P : PtsSig} : forall {Γ : Ctx P} {M M' A}, {{ Γ ⊢ M ≈ M' : A }} -> forall {Δ}, {{ ⊢ Δ ≈ Γ }} -> {{ Δ ⊢ M ≈ M' : A }}
+ctxeq_exp_eq_helper {P : PtsSig} : forall {Γ : ctx P} {M M' A}, {{ Γ ⊢ M ≈ M' : A }} -> forall {Δ}, {{ ⊢ Δ ≈ Γ }} -> {{ Δ ⊢ M ≈ M' : A }}
 with
-ctxeq_typ_helper {P : PtsSig} : forall {Γ : Ctx P} {A}, {{ Γ ⊢ A }} -> forall {Δ}, {{ ⊢ Δ ≈ Γ }} -> {{ Δ ⊢ A }}
+ctxeq_typ_helper {P : PtsSig} : forall {Γ : ctx P} {A}, {{ Γ ⊢ A }} -> forall {Δ}, {{ ⊢ Δ ≈ Γ }} -> {{ Δ ⊢ A }}
 with
-ctxeq_typ_eq_helper {P : PtsSig} : forall {Γ : Ctx P} {A B}, {{ Γ ⊢ A ≈ B }} -> forall {Δ}, {{ ⊢ Δ ≈ Γ }} -> {{ Δ ⊢ A ≈ B }}
+ctxeq_typ_eq_helper {P : PtsSig} : forall {Γ : ctx P} {A B}, {{ Γ ⊢ A ≈ B }} -> forall {Δ}, {{ ⊢ Δ ≈ Γ }} -> {{ Δ ⊢ A ≈ B }}
 with
-ctxeq_sub_helper {P : PtsSig} : forall {Γ : Ctx P} {Γ' σ}, {{ Γ ⊢s σ : Γ' }} -> forall {Δ}, {{ ⊢ Δ ≈ Γ }} -> {{ Δ ⊢s σ : Γ' }}
+ctxeq_sub_helper {P : PtsSig} : forall {Γ : ctx P} {Γ' σ}, {{ Γ ⊢s σ : Γ' }} -> forall {Δ}, {{ ⊢ Δ ≈ Γ }} -> {{ Δ ⊢s σ : Γ' }}
 with
-ctxeq_sub_eq_helper {P : PtsSig} : forall {Γ : Ctx P} {Γ' σ σ'}, {{ Γ ⊢s σ ≈ σ' : Γ' }} -> forall {Δ}, {{ ⊢ Δ ≈ Γ }} -> {{ Δ ⊢s σ ≈ σ' : Γ' }}.
+ctxeq_sub_eq_helper {P : PtsSig} : forall {Γ : ctx P} {Γ' σ σ'}, {{ Γ ⊢s σ ≈ σ' : Γ' }} -> forall {Δ}, {{ ⊢ Δ ≈ Γ }} -> {{ Δ ⊢s σ ≈ σ' : Γ' }}.
 Proof with mautosolve.
   all: inversion_clear 1;
     (on_all_hyp: gen_ctxeq_helper_IH (@ctxeq_exp_helper P) (@ctxeq_exp_eq_helper P) (@ctxeq_typ_helper P) (@ctxeq_typ_eq_helper P) (@ctxeq_sub_helper P) (@ctxeq_sub_eq_helper P));
@@ -55,96 +55,115 @@ Proof with mautosolve.
 
   (** Exp well-formedness cases *)
   (** Π and λ cases *)
-  2,3: assert {{ Δ ⊢ B : Sort@s1 }} by mauto; econstructor; mauto.
+  1,2,3: assert {{ Δ ⊢ B : Sort@s1 }} by mauto; econstructor; mauto.
   
   (** Variable case *)
-  - assert (exists B, {{ #i : B :: Sort@s ∈ Δ }} /\ {{ Δ ⊢ B ≈ A : Sort@s }} /\ {{ Δ ⊢ A : Sort@s }}) by mauto.
+  - assert (exists B, {{ #x : B :: Sort@s ∈ Δ }} /\ {{ Γ ⊢ A ≈ B : Sort@s }} /\ {{ Δ ⊢ A ≈ B : Sort@s }} /\ {{ Δ ⊢ A : Sort@s }}) by mauto.
     destruct_conjs.
-    eapply wf_exp_conv; mauto 2.    
-
-  (** Function application case *)  
-  - assert {{ Δ ⊢ N : B }} by mauto.
-    assert {{ Δ ⊢ M0 : Π r B C }} by mauto.
-    assert {{ Δ ⊢ B : Sort@s1 }} by mauto.
-    assert {{ Δ, B::Sort@s1 ⊢ C : Sort@s2 }} by mauto.    
-    assert {{ Δ ⊢ Π r B C : Sort@s3 }} by mauto.
-    mauto 2.
+    eapply wf_exp_conv; mauto 3.
 
   (** Conversion case *)
   - assert {{ Δ ⊢ B ≈ A }} by mauto.
     assert {{ Δ ⊢ A }} by mauto.
     assert {{ Δ ⊢ M : B }} by mauto.
     mauto 2.
+
+
+
     
   (** Exp equality cases *)
-  (** β case *)
-  - assert {{ Δ ⊢ N : B }} by mauto.
-    assert {{ Δ ⊢ B : Sort@s1 }} by mauto.
-    assert {{ Δ, B::Sort@s1 ⊢ M0 : C }} by mauto.
-    mauto 2.
-
   (** Π congruence case *)
-  - assert {{ Δ ⊢ A1 : Sort@s1 }} by mauto.
-    assert {{ Δ ⊢ A1 ≈ A2 : Sort@s1 }} by mauto.
-    assert {{ Δ, A1::Sort@s1 ⊢ B1 ≈ B2 : Sort@s2 }} by mauto.
+  - assert {{ Δ ⊢ B : Sort@s1 }} by mauto.
+    assert {{ Δ ⊢ B ≈ B' : Sort@s1 }} by mauto.
+    assert {{ Δ, B::Sort@s1 ⊢ C ≈ C' : Sort@s2 }} by mauto.
     mauto 2.
 
   (** λ congruence case *)
-  - assert {{ Δ ⊢ A1 : Sort@s1 }} by mauto.
-    assert {{ Δ ⊢ A1 ≈ A2 : Sort@s1 }} by mauto.
-    assert {{ Δ, A1::Sort@s1 ⊢ M1 ≈ M2 : C }} by mauto.
+  - assert {{ Δ ⊢ B : Sort@s1 }} by mauto.
+    assert {{ Δ ⊢ B ≈ B' : Sort@s1 }} by mauto.
+    assert {{ Δ, B::Sort@s1 ⊢ C : Sort@s2 }} by mauto.
+    assert {{ Δ, B::Sort@s1 ⊢ M0 ≈ M'0 : C }} by mauto.
     mauto 2.
-
+    
   (** Function application congruence case *)
-  - assert {{ Δ ⊢ N1 ≈ N2 : B }} by mauto.
-    assert {{ Δ ⊢ M1 ≈ M2 : Π r B C }} by mauto.
-    assert {{ Δ ⊢ Π r B C : Sort@s3 }} by mauto.
+  - assert {{ Δ ⊢ N ≈ N' : B }} by mauto.
+    assert {{ Δ ⊢ M0 ≈ M'0 : Π r B C }} by mauto.
+    assert {{ Δ ⊢ B : Sort@s1 }} by mauto.
+    assert {{ Δ, B::Sort@s1 ⊢ C : Sort@s2 }} by mauto.
+    mauto 2.
+    
+  (** β case *)
+  - assert {{ Δ ⊢ B : Sort@s1 }} by mauto.
+    assert {{ Δ, B::Sort@s1 ⊢ C : Sort@s2 }} by mauto.
+    assert {{ Δ, B::Sort@s1 ⊢ M0 : C }} by mauto.
+    assert {{ Δ ⊢ N : B }} by mauto.
     mauto 2.
 
-  (** sub_wf cases *)
+  (** η case *)
+  - assert {{ Δ ⊢ B : Sort@s1 }} by mauto.
+    assert {{ Δ, B::Sort@s1 ⊢ C : Sort@s2 }} by mauto.
+    assert {{ Δ ⊢ M : Π r B C }} by mauto.
+    mauto 2.
+
+  (** Variable reflexivity case *)
+  - assert (exists B, {{ #x : B :: Sort@s ∈ Δ }} /\ {{ Γ ⊢ A ≈ B : Sort@s }} /\ {{ Δ ⊢ A ≈ B : Sort@s }} /\ {{ Δ ⊢ A : Sort@s }}) by mauto.
+    destruct_conjs.
+    eapply wf_exp_eq_conv; mauto.
+
+  (** Variable weakening case *)
+  - inversion_clear HΓΔ.
+    assert {{ ⊢ Γ1, A0::Sort@s }} by mauto.
+    assert (exists B1, {{ #x : B1 :: Sort@s' ∈ Γ1 }} /\ {{ Γ0 ⊢ B ≈ B1 : Sort@s' }} /\ {{ Γ1 ⊢ B ≈ B1 : Sort@s' }} /\ {{ Γ1 ⊢ B : Sort@s' }}) by mauto.
+    destruct_conjs.
+    eapply wf_exp_eq_conv; mauto.
+
+  (** Conversion case *)
+  - assert {{ Δ ⊢ M ≈ M' : B }} by mauto.
+    assert {{ Δ ⊢ A }} by mauto.
+    assert {{ Δ ⊢ B ≈ A }} by mauto.
+    mauto 2.
+    
+  (** sub_wf cases (only weakening *)
   - inversion_clear HΓΔ.
     eapply wf_sub_conv; mauto.
 
-  (** Id expansion cases *)
+  (** Id expansion cases (only weakening reflexivity) *)
   - inversion_clear HΓΔ.
     mauto.
-
-  - inversion_clear HΓΔ.
-    eapply eq_sub_conv; mauto.    
 Qed.  (* I don't know why this Qed takes so long to check *)
 
 
-Corollary ctxeq_exp {P : PtsSig} : forall {Γ : Ctx P} {Δ M A}, {{ ⊢ Γ ≈ Δ }} -> {{ Γ ⊢ M : A }} -> {{ Δ ⊢ M : A }}.
+Corollary ctxeq_exp {P : PtsSig} : forall {Γ : ctx P} {Δ M A}, {{ ⊢ Γ ≈ Δ }} -> {{ Γ ⊢ M : A }} -> {{ Δ ⊢ M : A }}.
 Proof.
   intros; eapply ctxeq_exp_helper; mauto.
 Qed.
 
-Corollary ctxeq_exp_eq {P : PtsSig} : forall {Γ : Ctx P} {Δ M M' A}, {{ ⊢ Γ ≈ Δ }} -> {{ Γ ⊢ M ≈ M' : A }} -> {{ Δ ⊢ M ≈ M' : A }}.
+Corollary ctxeq_exp_eq {P : PtsSig} : forall {Γ : ctx P} {Δ M M' A}, {{ ⊢ Γ ≈ Δ }} -> {{ Γ ⊢ M ≈ M' : A }} -> {{ Δ ⊢ M ≈ M' : A }}.
 Proof.
   intros; eapply ctxeq_exp_eq_helper; mauto.
 Qed.
 
-Corollary ctxeq_typ {P : PtsSig} : forall {Γ : Ctx P} {Δ A}, {{ ⊢ Γ ≈ Δ }} -> {{ Γ ⊢ A }} -> {{ Δ ⊢ A }}.
+Corollary ctxeq_typ {P : PtsSig} : forall {Γ : ctx P} {Δ A}, {{ ⊢ Γ ≈ Δ }} -> {{ Γ ⊢ A }} -> {{ Δ ⊢ A }}.
 Proof.
   intros; eapply ctxeq_typ_helper; mauto.
 Qed.
 
-Corollary ctxeq_typ_eq {P : PtsSig} : forall {Γ : Ctx P} {Δ A B}, {{ ⊢ Γ ≈ Δ }} -> {{ Γ ⊢ A ≈ B }} -> {{ Δ ⊢ A ≈ B }}.
+Corollary ctxeq_typ_eq {P : PtsSig} : forall {Γ : ctx P} {Δ A B}, {{ ⊢ Γ ≈ Δ }} -> {{ Γ ⊢ A ≈ B }} -> {{ Δ ⊢ A ≈ B }}.
 Proof.
   intros; eapply ctxeq_typ_eq_helper; mauto.
 Qed.
 
-Corollary ctxeq_sub {P : PtsSig} : forall {Γ : Ctx P} {Δ σ Γ'}, {{ ⊢ Γ ≈ Δ }} -> {{ Γ ⊢s σ : Γ' }} -> {{ Δ ⊢s σ : Γ' }}.
+Corollary ctxeq_sub {P : PtsSig} : forall {Γ : ctx P} {Δ σ Γ'}, {{ ⊢ Γ ≈ Δ }} -> {{ Γ ⊢s σ : Γ' }} -> {{ Δ ⊢s σ : Γ' }}.
 Proof. intros; eapply ctxeq_sub_helper; mauto. Qed.
 
-Corollary ctxeq_sub_eq {P : PtsSig} : forall {Γ : Ctx P} {Δ σ σ' Γ'}, {{ ⊢ Γ ≈ Δ }} -> {{ Γ ⊢s σ ≈ σ' : Γ' }} -> {{ Δ ⊢s σ ≈ σ' : Γ' }}.
+Corollary ctxeq_sub_eq {P : PtsSig} : forall {Γ : ctx P} {Δ σ σ' Γ'}, {{ ⊢ Γ ≈ Δ }} -> {{ Γ ⊢s σ ≈ σ' : Γ' }} -> {{ Δ ⊢s σ ≈ σ' : Γ' }}.
 Proof. intros; eapply ctxeq_sub_eq_helper; mauto. Qed.
 
 #[export]
 Hint Resolve ctxeq_exp ctxeq_exp_eq ctxeq_sub ctxeq_sub_eq : mcpts.
 
 
-Lemma ctx_eq_trans {P : PtsSig} : forall {Γ0 Γ1 Γ2 : Ctx P}, {{ ⊢ Γ0 ≈ Γ1 }} -> {{ ⊢ Γ1 ≈ Γ2 }} -> {{ ⊢ Γ0 ≈ Γ2 }}.
+Lemma ctx_eq_trans {P : PtsSig} : forall {Γ0 Γ1 Γ2 : ctx P}, {{ ⊢ Γ0 ≈ Γ1 }} -> {{ ⊢ Γ1 ≈ Γ2 }} -> {{ ⊢ Γ0 ≈ Γ2 }}.
 Proof with mautosolve.
   intros * HΓ01.
   gen Γ2.
@@ -163,7 +182,7 @@ Qed.
 Hint Resolve ctx_eq_trans : mcpts.
 
 #[export]
-Instance wf_ctx_PER {P : PtsSig} : PER (@eq_ctx P).
+Instance wf_ctx_PER {P : PtsSig} : PER (@wf_ctx_eq P).
 Proof.
   split.
   - eauto using ctx_eq_sym.
@@ -173,28 +192,28 @@ Qed.
 
 
 Add Parametric Morphism {P : PtsSig} : (@wf_exp P)
-  with signature eq_ctx ==> eq ==> eq ==> iff as ctxeq_exp_morphism.
+  with signature wf_ctx_eq ==> eq ==> eq ==> iff as ctxeq_exp_morphism.
 Proof.
   intros. split; mauto 3.
 Qed.
 
 
-Add Parametric Morphism {P : PtsSig} : (@eq_exp P)
-  with signature eq_ctx ==> eq ==> eq ==> eq ==> iff as ctxeq_exp_eq_morphism.
+Add Parametric Morphism {P : PtsSig} : (@wf_exp_eq P)
+  with signature wf_ctx_eq ==> eq ==> eq ==> eq ==> iff as ctxeq_exp_eq_morphism.
 Proof.
   intros. split; mauto 3.
 Qed.
 
 
 Add Parametric Morphism {P : PtsSig} : (@wf_sub P)
-  with signature eq_ctx ==> eq ==> eq ==> iff as ctxeq_sub_morphism.
+  with signature wf_ctx_eq ==> eq ==> eq ==> iff as ctxeq_sub_morphism.
 Proof.
   intros. split; mauto 3.
 Qed.
 
 
-Add Parametric Morphism {P : PtsSig} : (@eq_sub P)
-  with signature eq_ctx ==> eq ==> eq ==> eq ==> iff as ctxeq_sub_eq_morphism.
+Add Parametric Morphism {P : PtsSig} : (@wf_sub_eq P)
+  with signature wf_ctx_eq ==> eq ==> eq ==> eq ==> iff as ctxeq_sub_eq_morphism.
 Proof.
   intros. split; mauto 3.
 Qed.
