mechanization/theories/Core/Syntactic/System/Lemmas.v
@@ -5,6 +5,993 @@ Import Syntax_Notations.
 
 (** ** Basic Context Properties *)
 
+Lemma ctx_lookup_lt {P : PtsSig} : forall {Γ : ctx P} {A x K},
+    {{ #x : A :: K ∈ Γ }} ->
+    x < length Γ.
+Proof.
+  induction 1; simpl; lia.
+Qed.
+#[export]
+Hint Resolve ctx_lookup_lt : mcpts.
+
+Lemma functional_ctx_lookup_typ {P : PtsSig} : forall {Γ : ctx P} {A A' x K K'},
+    {{ #x : A :: K ∈ Γ }} ->
+    {{ #x : A' :: K' ∈ Γ }} ->
+    A = A'.
+Proof with mautosolve.
+  intros * Hx Hx'; gen K' A'.
+  induction Hx as [|* ? IHHx]; intros; inversion_clear Hx';
+    f_equal;
+    intuition.
+Qed.
+
+Lemma functional_ctx_lookup_kd {P : PtsSig} : forall {Γ : ctx P} {A A' x K K'},
+    {{ #x : A :: K ∈ Γ }} ->
+    {{ #x : A' :: K' ∈ Γ }} ->
+    K = K'.
+Proof with mautosolve.
+  intros * Hx Hx'; gen K' A'. dependent induction Hx; intros.
+  - inversion_clear Hx'. auto. 
+  - inversion_clear Hx'; auto.
+    eapply IHHx; mauto.
+Qed.
+
+Lemma functional_ctx_lookup {P : PtsSig} : forall {Γ : ctx P} {A A' x K K'},
+    {{ #x : A :: K ∈ Γ }} ->
+    {{ #x : A' :: K' ∈ Γ }} ->
+    A = A' /\ K = K'.
+Proof with mautosolve.
+  intros; split.
+  - eapply functional_ctx_lookup_typ; mauto.
+  - eapply functional_ctx_lookup_kd; mauto.
+Qed.
+
+Lemma ctx_decomp {P : PtsSig} : forall {Γ : ctx P} {A K}, {{ ⊢ Γ, A::K }} -> {{ ⊢ Γ }} /\ {{ Γ ⊢ A : K }}.
+Proof with now eauto.
+  inversion 1...
+Qed.
+
+#[export]
+Hint Resolve ctx_decomp : mcpts.
+
+Corollary ctx_decomp_left {P : PtsSig} : forall {Γ : ctx P} {A K}, {{ ⊢ Γ , A::K }} -> {{ ⊢ Γ }}.
+Proof with easy.
+  intros * ?%ctx_decomp...
+Qed.
+
+Corollary ctx_decomp_right {P : PtsSig} : forall {Γ : ctx P} {A K}, {{ ⊢ Γ, A::K }} -> {{ Γ ⊢ A : K }}.
+Proof with easy.
+  intros * ?%ctx_decomp...
+Qed.
+
+#[export]
+Hint Resolve ctx_decomp_left ctx_decomp_right : mcpts.
+
+(** ** Core Presuppositions *)
+
+(** *** Context Presuppositions *)
+
+Lemma presup_ctx_eq {P : PtsSig} : forall {Γ Δ : ctx P}, {{ ⊢ Γ ≈ Δ }} -> {{ ⊢ Γ }} /\ {{ ⊢ Δ }}.
+Proof with mautosolve.
+  induction 1; destruct_pairs...
+Qed.
+
+Corollary presup_ctx_eq_left {P : PtsSig} : forall {Γ Δ : ctx P}, {{ ⊢ Γ ≈ Δ }} -> {{ ⊢ Γ }}.
+Proof with easy.
+  intros * ?%presup_ctx_eq...
+Qed.
+
+Corollary presup_ctx_eq_right {P : PtsSig} : forall {Γ Δ : ctx P}, {{ ⊢ Γ ≈ Δ }} -> {{ ⊢ Δ }}.
+Proof with easy.
+  intros * ?%presup_ctx_eq...
+Qed.
+
+#[export]
+Hint Resolve presup_ctx_eq presup_ctx_eq_left presup_ctx_eq_right : mcpts.
+
+Lemma presup_sub {P : PtsSig} : forall {Γ : ctx P} {Δ σ}, {{ Γ ⊢s σ : Δ }} -> {{ ⊢ Γ }} /\ {{ ⊢ Δ }}.
+Proof with mautosolve.
+  induction 1; destruct_pairs...
+Qed.
+
+Corollary presup_sub_left {P : PtsSig} : forall {Γ : ctx P} {Δ σ}, {{ Γ ⊢s σ : Δ }} -> {{ ⊢ Γ }}.
+Proof with easy.
+  intros * ?%presup_sub...
+Qed.
+
+Corollary presup_sub_right {P : PtsSig} : forall {Γ : ctx P} {Δ σ}, {{ Γ ⊢s σ : Δ }} -> {{ ⊢ Δ }}.
+Proof with easy.
+  intros * ?%presup_sub...
+Qed.
+
+#[export]
+Hint Resolve presup_sub presup_sub_left presup_sub_right : mcpts.
+
+(** With [presup_sub], we can prove similar for [exp]. *)
+
+Lemma presup_exp_ctx {P : PtsSig} : forall {Γ : ctx P} {M A}, {{ Γ ⊢ M : A }} -> {{ ⊢ Γ }}.
+Proof with mautosolve.
+  induction 1...
+Qed.
+
+#[export]
+Hint Resolve presup_exp_ctx : mcpts.
+
+(** and other presuppositions about context well-formedness. *)
+
+Lemma presup_sub_eq_ctx {P : PtsSig} : forall {Γ : ctx P} {Δ σ σ'}, {{ Γ ⊢s σ ≈ σ' : Δ }} -> {{ ⊢ Γ }} /\ {{ ⊢ Δ }}.
+Proof with mautosolve.
+  induction 1; destruct_pairs...
+Qed.
+
+Corollary presup_sub_eq_ctx_left {P : PtsSig} : forall {Γ : ctx P} {Δ σ σ'}, {{ Γ ⊢s σ ≈ σ' : Δ }} -> {{ ⊢ Γ }}.
+Proof with easy.
+  intros * ?%presup_sub_eq_ctx...
+Qed.
+
+Corollary presup_sub_eq_ctx_right {P : PtsSig} : forall {Γ : ctx P} {Δ σ σ'}, {{ Γ ⊢s σ ≈ σ' : Δ }} -> {{ ⊢ Δ }}.
+Proof with easy.
+  intros * ?%presup_sub_eq_ctx...
+Qed.
+
+#[export]
+Hint Resolve presup_sub_eq_ctx presup_sub_eq_ctx_left presup_sub_eq_ctx_right : mcpts.
+
+Lemma presup_exp_eq_ctx {P : PtsSig} : forall {Γ : ctx P} {M M' A}, {{ Γ ⊢ M ≈ M' : A }} -> {{ ⊢ Γ }}.
+Proof with mautosolve 2.
+  induction 1...
+Qed.
+
+#[export]
+Hint Resolve presup_exp_eq_ctx : mcpts.
+
+(** *** Immediate Results of Context Presuppositions *)
+
+(** Recover some rules we had before adding subtyping.
+    Rest are recovered after presupposition lemmas (in SystemOpt). *)
+
+Lemma wf_conv {P : PtsSig} : forall (Γ : ctx P) M A A',
+    {{ Γ ⊢ M : A }} ->
+    (** The next argument will be removed in SystemOpt *)
+    {{ Γ ⊢ A' }} ->
+    {{ Γ ⊢ A ≈ A' }} ->
+    {{ Γ ⊢ M : A' }}.
+Proof. mauto. Qed.
+
+#[export]
+Hint Resolve wf_conv : mcpts.
+
+Lemma wf_sub_conv {P : PtsSig} : forall (Γ : ctx P) σ Δ Δ',
+  {{ Γ ⊢s σ : Δ }} ->
+  {{ ⊢ Δ ≈ Δ' }} ->
+  {{ Γ ⊢s σ : Δ' }}.
+Proof. mauto. Qed.
+
+#[export]
+Hint Resolve wf_sub_conv : mcpts.
+
+Lemma wf_exp_eq_conv {P : PtsSig} : forall (Γ : ctx P) M M' A A',
+   {{ Γ ⊢ M ≈ M' : A }} ->
+   (** The next argument will be removed in SystemOpt *)
+   {{ Γ ⊢ A' }} ->
+   {{ Γ ⊢ A ≈ A' }} ->
+   {{ Γ ⊢ M ≈ M' : A' }}.
+Proof. mauto. Qed.
+
+#[export]
+Hint Resolve wf_exp_eq_conv : mcpts.
+
+Lemma wf_sub_eq_conv {P : PtsSig} : forall (Γ : ctx P) σ σ' Δ Δ',
+    {{ Γ ⊢s σ ≈ σ' : Δ }} ->
+    {{ ⊢ Δ ≈ Δ' }} ->
+    {{ Γ ⊢s σ ≈ σ' : Δ' }}.
+Proof. mauto. Qed.
+
+#[export]
+Hint Resolve wf_sub_eq_conv : mcpts.
+
+Add Parametric Morphism {P : PtsSig} (Γ : ctx P) : (wf_sub_eq Γ)
+    with signature wf_ctx_eq ==> eq ==> eq ==> iff as wf_sub_eq_morphism_iff3.
+Proof.
+  intros Δ Δ' H **; split; [| symmetry in H]; mauto.
+Qed.
+
+(** We can prove some additional lemmas for type presuppositions as well. *)
+
+(** *** Additional Lemmas for Syntactic PERs *)
+
+Lemma exp_eq_refl {P : PtsSig} : forall {Γ : ctx P} {M A},
+    {{ Γ ⊢ M : A }} ->
+    {{ Γ ⊢ M ≈ M : A }}.
+Proof. mauto. Qed.
+
+#[export]
+Hint Resolve exp_eq_refl : mcpts.
+
+(* Lemma exp_eq_trans_typ_max : forall {Γ i i' A A' A''}, *)
+(*     {{ Γ ⊢ A ≈ A' : Type@i }} -> *)
+(*     {{ Γ ⊢ A' ≈ A'' : Type@i' }} -> *)
+(*     {{ Γ ⊢ A ≈ A'' : Type@(max i i') }}. *)
+(* Proof with mautosolve 4. *)
+(*   intros. *)
+(*   assert {{ Γ ⊢ A ≈ A' : Type@(max i i') }} by eauto using lift_exp_eq_max_left. *)
+(*   assert {{ Γ ⊢ A' ≈ A'' : Type@(max i i') }} by eauto using lift_exp_eq_max_right... *)
+(* Qed. *)
+
+(* #[export] *)
+(* Hint Resolve exp_eq_trans_typ_max : mcpts. *)
+
+Lemma sub_eq_refl {P : PtsSig} : forall {Γ : ctx P} {σ Δ},
+    {{ Γ ⊢s σ : Δ }} ->
+    {{ Γ ⊢s σ ≈ σ : Δ }}.
+Proof. mauto. Qed.
+
+#[export]
+Hint Resolve sub_eq_refl : mcpts.
+
+Lemma ctx_eq_refl {P : PtsSig} : forall {Γ : ctx P},
+    {{ ⊢ Γ }} ->
+    {{ ⊢ Γ ≈ Γ }}.
+Proof.
+  induction 1; mauto 4.
+Qed.
+
+#[export]
+Hint Resolve ctx_eq_refl : mcpts.
+
+(** *** Lemmas for [exp] of [{{{ Type@i }}}] *)
+
+Lemma exp_sub_typ {P : PtsSig} : forall {Δ : ctx P} {Γ A σ s},
+    {{ Δ ⊢ A : Sort@s }} ->
+    {{ Γ ⊢s σ : Δ }} ->
+    {{ Γ ⊢ A[σ] : Sort@s }}.
+Proof with mautosolve 3.
+  intros.
+  econstructor; mauto 3.
+Qed.
+
+#[export]
+Hint Resolve exp_sub_typ : mcpts.
+
+Lemma presup_ctx_lookup_typ {P : PtsSig} : forall {Γ : ctx P} {A x K},
+    {{ ⊢ Γ }} ->
+    {{ #x : A :: K ∈ Γ }} ->
+    {{ Γ ⊢ A : K }} /\ exists s, K = {{{ Sort@s }}}.
+Proof with mautosolve 4.
+  intros * HΓ.
+  induction 1; inversion_clear HΓ; split; mauto 4;
+    assert ({{ Γ ⊢ A : K }} /\ exists s, K = {{{ Sort@s }}}) by (eapply IHctx_lookup; mauto 2);
+    destruct_conjs; subst; mauto 4.
+Qed.
+
+#[export]
+Hint Resolve presup_ctx_lookup_typ : mcpts.
+
+Lemma exp_eq_sub_cong_typ1 {P : PtsSig} : forall {Δ : ctx P} {Γ A A' σ},
+    {{ Δ ⊢ A ≈ A' }} ->
+    {{ Γ ⊢s σ : Δ }} ->
+    {{ Γ ⊢ A[σ] ≈ A'[σ] }}.
+Proof with mautosolve 3.
+  intros.
+  econstructor...
+Qed.
+
+Lemma exp_eq_sub_cong_typ2' {P : PtsSig} : forall {Δ : ctx P} {Γ A σ τ},
+    {{ Δ ⊢ A }} ->
+    {{ Γ ⊢s σ : Δ }} ->
+    {{ Γ ⊢s σ ≈ τ : Δ }} ->
+    {{ Γ ⊢ A[σ] ≈ A[τ] }}.
+Proof with mautosolve 3.
+  intros.
+  econstructor...
+Qed.
+
+Lemma exp_eq_sub_compose_typ {P : PtsSig} : forall {Ψ : ctx P} {Δ Γ A σ τ},
+    {{ Ψ ⊢ A }} ->
+    {{ Δ ⊢s σ : Ψ }} ->
+    {{ Γ ⊢s τ : Δ }} ->
+    {{ Γ ⊢ A[σ][τ] ≈ A[σ∘τ] }}.
+Proof with mautosolve 3.
+  intros.
+  econstructor...
+Qed.
+
+#[export]
+Hint Resolve exp_eq_sub_cong_typ1 exp_eq_sub_cong_typ2' exp_eq_sub_compose_typ : mcpts.
+
+Lemma exp_eq_sub_compose_weaken_extend_typ {P : PtsSig} : forall {Γ : ctx P} {σ Δ A B M s},
+    {{ Γ ⊢s σ : Δ }} ->
+    {{ Δ ⊢ A }} ->
+    {{ Δ ⊢ B : Sort@s }} ->
+    {{ Γ ⊢ M : B[σ] }} ->
+    {{ Γ ⊢ A[Wk][σ,,M] ≈ A[σ] }}.
+Proof with mautosolve 3.
+  intros.
+  assert {{ Δ, B::Sort@s ⊢s Wk : Δ }} by mauto 4.
+  transitivity {{{ A[Wk∘(σ,,M)] }}}; [mautosolve 4 |].
+  eapply exp_eq_sub_cong_typ2'...
+Qed.
+
+#[export]
+Hint Resolve exp_eq_sub_compose_weaken_extend_typ : mcpts.
+
+Lemma exp_eq_sub_compose_weaken_id_extend_typ {P : PtsSig} : forall {Γ : ctx P} {A s B M},
+    {{ Γ ⊢ A }} ->
+    {{ Γ ⊢ B : Sort@s }} ->
+    {{ Γ ⊢ M : B }} ->
+    {{ Γ ⊢ A[Wk][Id,,M] ≈ A }}.
+Proof with mautosolve 4.
+  intros.
+  assert {{ Γ ⊢ B[Id] : Sort@s }} by mauto 4.
+  assert {{ Γ ⊢ B ≈ B[Id] }} by mauto 4.
+  assert {{ Γ ⊢ M : B[Id] }} by (eapply wf_conv; mauto 2).
+  transitivity {{{ A[Id] }}}...
+Qed.
+
+#[export]
+Hint Resolve exp_eq_sub_compose_weaken_id_extend_typ : mcpts.
+
+Lemma exp_eq_sub_compose_double_weaken_double_extend_typ {P : PtsSig} : forall {Γ : ctx P} {σ Δ A s1 B M s2 C N},
+    {{ Γ ⊢s σ : Δ }} ->
+    {{ Δ ⊢ A }} ->
+    {{ Δ ⊢ B : Sort@s1 }} ->
+    {{ Γ ⊢ M : B[σ] }} ->
+    {{ Δ, B::Sort@s1 ⊢ C : Sort@s2 }} ->
+    {{ Γ ⊢ N : C[σ,,M] }} ->
+    {{ Γ ⊢ A[Wk∘Wk][σ,,M,,N] ≈ A[σ] }}.
+Proof with mautosolve 4.
+  intros.
+  assert {{ Δ, B::Sort@s1 ⊢s Wk : Δ }} by mauto 4.
+  assert {{ Δ, B::Sort@s1, C::Sort@s2 ⊢s Wk : Δ, B::Sort@s1 }} by mauto 4.
+  transitivity {{{ A[Wk][Wk][σ,,M,,N] }}}; [eapply exp_eq_sub_cong_typ1; mautosolve 3 |].
+  transitivity {{{ A[Wk][σ,,M] }}}...
+Qed.
+
+#[export]
+Hint Resolve exp_eq_sub_compose_double_weaken_double_extend_typ : mcpts.
+
+Lemma exp_eq_sub_compose_double_weaken_id_double_extend_typ {P : PtsSig} : forall {Γ : ctx P} {A s1 B M s2 C N},
+    {{ Γ ⊢ A }} ->
+    {{ Γ ⊢ B : Sort@s1 }} ->
+    {{ Γ ⊢ M : B }} ->
+    {{ Γ, B::Sort@s1 ⊢ C : Sort@s2 }} ->
+    {{ Γ ⊢ N : C[Id,,M] }} ->
+    {{ Γ ⊢ A[Wk∘Wk][Id,,M,,N] ≈ A }}.
+Proof with mautosolve 4.
+  intros.
+  assert {{ Γ ⊢ B[Id] : Sort@s1 }} by mauto 4.
+  assert {{ Γ ⊢ B ≈ B[Id] }} by mauto 4.
+  assert {{ Γ ⊢ M : B[Id] }} by (eapply wf_conv; mauto 2).
+  transitivity {{{ A[Id] }}}...
+Qed.
+
+#[export]
+Hint Resolve exp_eq_sub_compose_double_weaken_id_double_extend_typ : mcpts.
+
+Lemma exp_eq_typ_sub_sub {P : PtsSig} : forall {Γ : ctx P} {Δ Ψ σ τ s},
+    {{ Δ ⊢s σ : Ψ }} ->
+    {{ Γ ⊢s τ : Δ }} ->
+    {{ Γ ⊢ Sort@s[σ][τ] ≈ Sort@s }}.
+Proof. mauto. Qed.
+
+#[export]
+Hint Resolve exp_eq_typ_sub_sub : mcpts.
+#[export]
+Hint Rewrite -> @exp_eq_sub_compose_typ @exp_eq_typ_sub_sub using mauto 4 : mcpts.
+
+Lemma vlookup_0_typ {P : PtsSig} : forall {Γ : ctx P} {s1 s2},
+    Ax P s1 s2 ->
+    {{ ⊢ Γ }} ->
+    {{ Γ, Sort@s1::Sort@s2 ⊢ #0 : Sort@s1 }}.
+Proof with mautosolve 4.
+  intros.
+  eapply wf_conv; mauto 4.
+  econstructor...
+Qed.
+
+Lemma vlookup_1_typ {P : PtsSig} : forall {Γ : ctx P} {s1 s2 A s3},
+    Ax P s1 s2 ->
+    {{ Γ, Sort@s1::Sort@s2 ⊢ A : Sort@s3 }} ->
+    {{ Γ, Sort@s1::Sort@s2, A::Sort@s3 ⊢ #1 : Sort@s1 }}.
+Proof with mautosolve 4.
+  intros.
+  assert {{ Γ, Sort@s1::Sort@s2 ⊢s Wk : Γ }} by mauto 4.
+  assert {{ Γ, Sort@s1::Sort@s2, A::Sort@s3 ⊢s Wk : Γ, Sort@s1::Sort@s2 }} by mauto 4.
+  eapply wf_conv...
+Qed.
+
+#[export]
+Hint Resolve vlookup_0_typ vlookup_1_typ : mcpts.
+
+Lemma exp_sub_typ_helper {P : PtsSig} : forall {Γ : ctx P} {σ Δ M s},
+    {{ Γ ⊢s σ : Δ }} ->
+    {{ Γ ⊢ M : Sort@s }} ->
+    {{ Γ ⊢ M : Sort@s[σ] }}.
+Proof.
+  intros.
+  do 2 (econstructor; mauto 4).
+Qed.
+
+#[export]
+Hint Resolve exp_sub_typ_helper : mcpts.
+
+Lemma exp_eq_var_0_sub_typ {P : PtsSig} : forall {Γ : ctx P} {σ Δ M s1 s2},
+    Ax P s1 s2 ->
+    {{ Γ ⊢s σ : Δ }} ->
+    {{ Γ ⊢ M : Sort@s1 }} ->
+    {{ Γ ⊢ #0[σ,,M] ≈ M : Sort@s1 }}.
+Proof with mautosolve 4.
+  intros.
+  eapply wf_exp_eq_conv with (A := {{{ Sort@s1[σ] }}}); mauto 3.
+  econstructor...
+Qed.
+
+Lemma exp_eq_var_1_sub_typ {P : PtsSig} : forall {Γ : ctx P} {σ Δ A s1 M s2 s3},
+    {{ Γ ⊢s σ : Δ }} ->
+    {{ Δ ⊢ A : Sort@s1 }} ->
+    {{ Γ ⊢ M : A[σ] }} ->
+    {{ #0 : Sort@s2[Wk] :: Sort@s3 ∈ Δ }} ->
+    {{ Γ ⊢ #1[σ,,M] ≈ #0[σ] : Sort@s2 }}.
+Proof with mautosolve 4.
+  inversion 4 as [? ? Δ'|]; subst.
+  assert {{ ⊢ Δ' }} by mauto 4.
+  assert {{ Δ', Sort@s2::Sort@s3 ⊢s Wk : Δ' }} by mauto 4.
+  eapply wf_exp_eq_conv...
+Qed.
+
+#[export]
+Hint Resolve exp_eq_var_0_sub_typ exp_eq_var_1_sub_typ : mcpts.
+#[export]
+Hint Rewrite -> @exp_eq_var_0_sub_typ @exp_eq_var_1_sub_typ : mcpts.
+
+Lemma exp_eq_var_0_weaken_typ {P : PtsSig} : forall {Γ : ctx P} {A s1 s2 s3},
+    {{ ⊢ Γ, A::Sort@s1 }} ->
+    {{ #0 : Sort@s2[Wk]::Sort@s3 ∈ Γ }} ->
+    {{ Γ, A::Sort@s1 ⊢ #0[Wk] ≈ #1 : Sort@s2 }}.
+Proof with mautosolve 3.
+  inversion_clear 1.
+  inversion 1 as [? ? Γ'|]; subst.
+  assert {{ ⊢ Γ' }} by mauto.
+  assert {{ Γ', Sort@s2::Sort@s3 ⊢s Wk : Γ' }} by mauto 4.
+  assert {{ Γ', Sort@s2::Sort@s3, A::Sort@s1 ⊢s Wk : Γ', Sort@s2::Sort@s3 }} by mauto 4.
+  eapply wf_exp_eq_conv...
+Qed.
+
+#[export]
+Hint Resolve exp_eq_var_0_weaken_typ : mcpts.
+
+Lemma sub_extend_typ {P : PtsSig} : forall {Γ : ctx P} {σ Δ M s1 s2},
+    Ax P s1 s2 ->
+    {{ Γ ⊢s σ : Δ }} ->
+    {{ Γ ⊢ M : Sort@s1 }} ->
+    {{ Γ ⊢s σ,,M : Δ, Sort@s1::Sort@s2 }}.
+Proof with mautosolve 4.
+  intros.
+  econstructor...
+Qed.
+
+#[export]
+Hint Resolve sub_extend_typ : mcpts.
+
+Lemma sub_eq_extend_cong_typ {P : PtsSig} : forall {Γ : ctx P} {σ σ' Δ M M' s1 s2},
+    Ax P s1 s2 ->
+    {{ Γ ⊢s σ : Δ }} ->
+    {{ Γ ⊢s σ ≈ σ' : Δ }} ->
+    {{ Γ ⊢ M ≈ M' : Sort@s1 }} ->
+    {{ Γ ⊢s σ,,M ≈ σ',,M' : Δ, Sort@s1::Sort@s2 }}.
+Proof with mautosolve 4.
+  intros.
+  econstructor; mauto 3.
+  eapply wf_exp_eq_conv...
+Qed.
+
+Lemma sub_eq_extend_compose_typ {P : PtsSig} : forall {Γ : ctx P} {τ Γ' σ Γ'' A s1 s2 s3 M},
+    Ax P s2 s3 ->
+    {{ Γ' ⊢s σ : Γ'' }} ->
+    {{ Γ'' ⊢ A : Sort@s1 }} ->
+    {{ Γ' ⊢ M : Sort@s2 }} ->
+    {{ Γ ⊢s τ : Γ' }} ->
+    {{ Γ ⊢s (σ,,M)∘τ ≈ (σ∘τ),,M[τ] : Γ'', Sort@s2::Sort@s3 }}.
+Proof with mautosolve 4.
+  intros.
+  econstructor...
+Qed.
+
+Lemma sub_eq_p_extend_typ {P : PtsSig} : forall {Γ : ctx P} {σ Γ' M s1 s2},
+    Ax P s1 s2 ->
+    {{ Γ' ⊢s σ : Γ }} ->
+    {{ Γ' ⊢ M : Sort@s1 }} ->
+    {{ Γ' ⊢s Wk∘(σ,,M) ≈ σ : Γ }}.
+Proof with mautosolve 4.
+  intros.
+  assert {{ Γ ⊢ Sort@s1 : Sort@s2 }} by mauto.
+  econstructor; mauto 3.
+Qed.
+
+#[export]
+Hint Resolve sub_eq_extend_cong_typ sub_eq_extend_compose_typ sub_eq_p_extend_typ : mcpts.
+
+
+Lemma exp_eq_sub_sub_compose_cong_typ {P : PtsSig} : forall {Γ : ctx P} {Δ Δ' Ψ σ τ σ' τ' A},
+    {{ Ψ ⊢ A }} ->
+    {{ Δ ⊢s σ : Ψ }} ->
+    {{ Δ' ⊢s σ' : Ψ }} ->
+    {{ Γ ⊢s τ : Δ }} ->
+    {{ Γ ⊢s τ' : Δ' }} ->
+    {{ Γ ⊢s σ∘τ ≈ σ'∘τ' : Ψ }} ->
+    {{ Γ ⊢ A[σ][τ] ≈ A[σ'][τ'] }}.
+Proof with mautosolve 4.
+  intros.
+  assert {{ Γ ⊢ A[σ][τ] ≈ A[σ∘τ] }} by mauto.
+  assert {{ Γ ⊢ A[σ∘τ] ≈ A[σ'∘τ'] }} by mauto.
+  enough {{ Γ ⊢ A[σ'∘τ'] ≈ A[σ'][τ'] }}...
+Qed.
+
+#[export]
+Hint Resolve exp_eq_sub_sub_compose_cong_typ : mcpts.
+
+
+(** *** Other Tedious Lemmas *)
+
+Lemma sub_eq_weaken_var0_id {P : PtsSig} : forall {Γ : ctx P} {A s},
+    {{ Γ ⊢ A : Sort@s }} ->
+    {{ Γ, A::Sort@s ⊢s Wk,,#0 ≈ Id : Γ, A::Sort@s }}.
+Proof with mautosolve 4.
+  intros * ?.
+  assert {{ ⊢ Γ, A::Sort@s }} by mauto 3.
+  assert {{ Γ, A::Sort@s ⊢s (Wk∘Id),,#0[Id] ≈ Id : Γ, A::Sort@s }} by mauto.
+  assert {{ Γ, A::Sort@s ⊢s Wk ≈ Wk∘Id : Γ }} by mauto.
+  enough {{ Γ, A::Sort@s ⊢ #0 ≈ #0[Id] : A[Wk] }}...
+Qed.
+
+#[export]
+Hint Resolve sub_eq_weaken_var0_id : mcpts.
+#[export]
+Hint Rewrite -> @sub_eq_weaken_var0_id using mauto 4 : mcpts.
+
+Lemma exp_eq_sub_sub_compose_cong {P : PtsSig} : forall {Γ : ctx P} {Δ Δ' Ψ σ τ σ' τ' M A s},
+    {{ Ψ ⊢ A : Sort@s }} ->
+    {{ Ψ ⊢ M : A }} ->
+    {{ Δ ⊢s σ : Ψ }} ->
+    {{ Δ' ⊢s σ' : Ψ }} ->
+    {{ Γ ⊢s τ : Δ }} ->
+    {{ Γ ⊢s τ' : Δ' }} ->
+    {{ Γ ⊢s σ∘τ ≈ σ'∘τ' : Ψ }} ->
+    {{ Γ ⊢ M[σ][τ] ≈ M[σ'][τ'] : A[σ∘τ] }}.
+Proof with mautosolve 4.
+  intros.
+  assert {{ Γ ⊢ A[σ∘τ] ≈ A[σ'∘τ'] : Sort@s }} by (eapply wf_exp_eq_conv; mauto).
+  assert {{ Γ ⊢ M[σ][τ] ≈ M[σ∘τ] : A[σ∘τ] }} by mauto.
+  assert {{ Γ ⊢ M[σ∘τ] ≈ M[σ'∘τ'] : A[σ∘τ] }} by mauto.
+  assert {{ Γ ⊢ M[σ'∘τ'] ≈ M[σ'][τ'] : A[σ'∘τ'] }} by mauto.
+  enough {{ Γ ⊢ M[σ'∘τ'] ≈ M[σ'][τ'] : A[σ∘τ] }} by mauto.
+  eapply wf_exp_eq_conv...
+Qed.
+
+#[export]
+Hint Resolve exp_eq_sub_sub_compose_cong : mcpts.
+
+Lemma ctxeq_ctx_lookup {P : PtsSig} : forall {Γ : ctx P} {Δ A x s},
+    {{ ⊢ Γ ≈ Δ }} ->
+    {{ #x : A :: Sort@s ∈ Γ }} ->
+    exists B,
+      {{ #x : B :: Sort@s ∈ Δ }} /\
+        {{ Γ ⊢ A ≈ B : Sort@s }} /\
+        {{ Δ ⊢ A ≈ B : Sort@s }} /\
+        {{ Δ ⊢ A : Sort@s }}.
+Proof with mautosolve.
+  intros * HΓΔ Hx; gen Δ.
+  induction Hx as [|* ? IHHx]; inversion_clear 1 as [|? ? ? ? ? HΓΔ'];
+    [|specialize (IHHx _ HΓΔ')]; destruct_conjs; eexists.
+  - split.
+    + econstructor; mauto.
+    + split.
+      * eapply wf_exp_eq_conv; mauto.
+      * split.
+        -- eapply wf_exp_eq_conv; mauto.
+        -- econstructor; mauto.
+  - split.
+    + econstructor; mauto.
+    + split.
+      * assert ({{ Γ ⊢ A : K }} /\ exists s', K = {{{ Sort@s' }}}) by (eapply presup_ctx_lookup_typ; mauto).
+        destruct_conjs; subst.
+        eapply wf_exp_eq_conv; mauto.
+      * split.
+        -- assert ({{ Δ0 ⊢ IHHx : K }} /\ exists s', K = {{{ Sort@s' }}}) by (eapply presup_ctx_lookup_typ; mauto).
+        destruct_conjs; subst.
+        eapply wf_exp_eq_conv; mauto.
+        -- assert ({{ Δ0 ⊢ IHHx : K }} /\ exists s', K = {{{ Sort@s' }}}) by (eapply presup_ctx_lookup_typ; mauto).
+           destruct_conjs; subst.
+           econstructor; mauto.           
+Qed.
+
+#[export]
+Hint Resolve ctxeq_ctx_lookup : mcpts.
+
+Lemma sub_id_on_typ {P : PtsSig} : forall {Γ : ctx P} {M A s},
+    {{ Γ ⊢ A : Sort@s }} ->
+    {{ Γ ⊢ M : A }} ->
+    {{ Γ ⊢ M : A[Id] }}.
+Proof with mautosolve 4.
+  intros.
+  eapply wf_conv with (A := A); mauto.
+Qed.
+
+#[export]
+Hint Resolve sub_id_on_typ : mcpts.
+
+Lemma sub_id_extend {P : PtsSig} : forall {Γ : ctx P} {M A s},
+    {{ Γ ⊢ A : Sort@s }} ->
+    {{ Γ ⊢ M : A }} ->
+    {{ Γ ⊢s Id,,M : Γ, A::Sort@s }}.
+Proof with mautosolve 4.
+  intros.
+  econstructor...
+Qed.
+
+#[export]
+Hint Resolve sub_id_extend : mcpts.
+
+Lemma sub_eq_id_on_typ {P : PtsSig} : forall {Γ : ctx P} {M M' A s},
+    {{ Γ ⊢ A : Sort@s }} ->
+    {{ Γ ⊢ M ≈ M' : A }} ->
+    {{ Γ ⊢ M ≈ M' : A[Id] }}.
+Proof with mautosolve 4.
+  intros.
+  eapply wf_exp_eq_conv; mauto.
+Qed.
+
+#[export]
+Hint Resolve sub_eq_id_on_typ : mcpts.
+
+Lemma sub_eq_id_extend_cong {P : PtsSig} : forall {Γ : ctx P} {M M' A s},
+    {{ Γ ⊢ A : Sort@s }} ->
+    {{ Γ ⊢ M ≈ M' : A }} ->
+    {{ Γ ⊢s Id,,M ≈ Id,,M' : Γ, A::Sort@s }}.
+Proof with mautosolve 4.
+  intros.
+  econstructor; mauto 3.
+Qed.
+
+#[export]
+Hint Resolve sub_eq_id_extend_cong : mcpts.
+
+Lemma sub_eq_p_id_extend {P : PtsSig} : forall {Γ : ctx P} {M A s},
+    {{ Γ ⊢ A : Sort@s }} ->
+    {{ Γ ⊢ M : A }} ->
+    {{ Γ ⊢s Wk∘(Id,,M) ≈ Id : Γ }}.
+Proof with mautosolve 4.
+  intros.
+  econstructor...
+Qed.
+
+#[export]
+Hint Resolve sub_eq_p_id_extend : mcpts.
+#[export]
+Hint Rewrite -> @sub_eq_p_id_extend using mauto 4 : mcpts.
+
+Lemma sub_q {P : PtsSig} : forall {Γ : ctx P} {A s σ Δ},
+    {{ Δ ⊢ A : Sort@s }} ->
+    {{ Γ ⊢s σ : Δ }} ->
+    {{ Γ, A[σ]::Sort@s ⊢s q σ : Δ, A::Sort@s }}.
+Proof with mautosolve 3.
+  intros.
+  assert {{ Γ ⊢ A[σ] : Sort@s }} by mauto 4.
+  assert {{ Γ, A[σ]::Sort@s ⊢s Wk : Γ }} by mauto 4.
+  assert {{ Γ, A[σ]::Sort@s ⊢ #0 : A[σ][Wk] }} by mauto 4.
+  econstructor; mauto 3.
+  eapply wf_conv; mauto.
+Qed.
+
+Lemma sub_q_typ {P : PtsSig} : forall {Γ σ Δ s1 s2},
+    Ax P s1 s2 ->
+    {{ Γ ⊢s σ : Δ }} ->
+    {{ Γ, Sort@s1::Sort@s2 ⊢s q σ : Δ, Sort@s1::Sort@s2 }}.
+Proof with mautosolve 4.
+  intros.
+  assert {{ ⊢ Γ }} by mauto 3.
+  assert {{ Γ, Sort@s1::Sort@s2 ⊢s Wk : Γ }} by mauto 4.
+  assert {{ Γ, Sort@s1::Sort@s2 ⊢s σ∘Wk : Δ }} by mauto 4.
+  assert {{ Γ, Sort@s1::Sort@s2 ⊢ #0 : Sort@s1 }}...
+Qed.
+
+#[export]
+Hint Resolve sub_q sub_q_typ : mcpts.
+
+Lemma sub_eq_id_extend_compose_sigma {P : PtsSig} : forall {Γ : ctx P} {M A σ Δ s},
+    {{ Γ ⊢s σ : Δ }} ->
+    {{ Δ ⊢ A : Sort@s }} ->
+    {{ Δ ⊢ M : A }} ->
+    {{ Γ ⊢s (Id,,M)∘σ ≈ σ,,M[σ] : Δ, A::Sort@s }}.
+Proof with mautosolve 4.
+  intros.
+  assert {{ Δ ⊢s Id : Δ }} by mauto.
+  assert {{ Δ ⊢ M : A[Id] }} by mauto.
+  assert {{ Γ ⊢s (Id,,M)∘σ ≈ (Id∘σ),,M[σ] : Δ, A::Sort@s }} by mauto 3.
+  assert {{ Γ ⊢ M[σ] : A[Id][σ] }} by mauto.
+  assert {{ Γ ⊢ A[Id][σ] ≈ A[Id∘σ] : Sort@s }} by (eapply wf_exp_eq_conv; mauto).
+  assert {{ Γ ⊢ M[σ] : A[Id∘σ] }} by (eapply wf_conv; mauto 4).
+  enough {{ Γ ⊢ M[σ] ≈ M[σ] : A[Id∘σ] }}...
+Qed.
+
+#[export]
+Hint Resolve sub_eq_id_extend_compose_sigma : mcpts.
+
+Lemma sub_eq_sigma_compose_weak_id_extend {P : PtsSig} : forall {Γ : ctx P} {M A s σ Δ},
+    {{ Γ ⊢ A : Sort@s }} ->
+    {{ Γ ⊢s σ : Δ }} ->
+    {{ Γ ⊢ M : A }} ->
+    {{ Γ ⊢s (σ∘Wk)∘(Id,,M) ≈ σ : Δ }}.
+Proof with mautosolve.
+  intros.
+  assert {{ Γ ⊢s Id,,M : Γ, A::Sort@s }} by mauto.
+  assert {{ Γ ⊢s (σ∘Wk)∘(Id,,M) ≈ σ∘(Wk∘(Id,,M)) : Δ }} by mauto 4.
+  assert {{ Γ ⊢s Wk∘(Id,,M) ≈ Id : Γ }} by mauto.
+  enough {{ Γ ⊢s σ∘(Wk∘ (Id,,M)) ≈ σ∘Id : Δ }} by mauto.
+  econstructor...
+Qed.
+
+#[export]
+Hint Resolve sub_eq_sigma_compose_weak_id_extend : mcpts.
+
+Lemma sub_eq_q_sigma_id_extend {P : PtsSig} : forall {Γ : ctx P} {M A s σ Δ},
+    {{ Δ ⊢ A : Sort@s }} ->
+    {{ Γ ⊢s σ : Δ }} ->
+    {{ Γ ⊢ M : A[σ] }} ->
+    {{ Γ ⊢s q σ∘(Id,,M) ≈ σ,,M : Δ, A::Sort@s }}.
+Proof with mautosolve 4.
+  intros.
+  assert {{ ⊢ Γ }} by mauto 3.
+  assert {{ Γ ⊢ A[σ] : Sort@s }} by mauto.
+  assert {{ Γ ⊢ M : A[σ] }} by mauto.
+  assert {{ Γ ⊢s Id,,M : Γ, A[σ]::Sort@s }} by mauto.
+  assert {{ Γ, A[σ]::Sort@s ⊢s Wk : Γ }} by mauto.
+  assert {{ Γ, A[σ]::Sort@s ⊢ #0 : A[σ][Wk] }} by mauto.
+  assert {{ Γ, A[σ]::Sort@s ⊢ #0 : A[σ∘Wk] }} by (eapply wf_conv; mauto 4).
+  assert {{ Γ ⊢s q σ∘(Id,,M) ≈ ((σ∘Wk)∘(Id,,M)),,#0[Id,,M] : Δ, A::Sort@s }} by mauto.
+  assert {{ Γ ⊢s (σ∘Wk)∘(Id,,M) ≈ σ : Δ }} by mauto.
+  assert {{ Γ ⊢ M : A[σ][Id] }} by mauto 4.
+  assert {{ Γ ⊢ #0[Id,,M] ≈ M : A[σ][Id] }} by mauto 3.
+  assert {{ Γ ⊢ #0[Id,,M] ≈ M : A[σ] }} by mauto.
+  enough {{ Γ ⊢ #0[Id,,M] ≈ M : A[(σ∘Wk)∘(Id,,M)] }} by mauto.
+  eapply wf_exp_eq_conv; mauto.
+Qed.
+
+#[export]
+Hint Resolve sub_eq_q_sigma_id_extend : mcpts.
+#[export]
+Hint Rewrite -> @sub_eq_q_sigma_id_extend using mauto 4 : mcpts.
+
+Lemma sub_eq_p_q_sigma {P : PtsSig} : forall {Γ : ctx P} {A s σ Δ},
+    {{ Δ ⊢ A : Sort@s }} ->
+    {{ Γ ⊢s σ : Δ }} ->
+    {{ Γ, A[σ]::Sort@s ⊢s Wk∘q σ ≈ σ∘Wk : Δ }}.
+Proof with mautosolve 3.
+  intros.
+  assert {{ Γ, A[σ]::Sort@s ⊢s Wk : Γ }} by mauto 4.
+  assert {{ Γ, A[σ]::Sort@s ⊢ #0 : A[σ][Wk] }} by mauto 3.
+  enough {{ Γ, A[σ]::Sort@s ⊢ #0 : A[σ∘Wk] }} by mauto.
+  eapply wf_conv; mauto.
+Qed.
+
+#[export]
+Hint Resolve sub_eq_p_q_sigma : mcpts.
+
+
+(** *** Lemmas for [wf_typ_eq] *)
+
+Fact wf_typ_eq_refl {P : PtsSig} : forall {Γ : ctx P} {A},
+    {{ Γ ⊢ A }} ->
+    {{ Γ ⊢ A ≈ A }}.
+Proof. mauto. Qed.
+
+#[export]
+Hint Resolve wf_typ_eq_refl : mcpts.
+
+Lemma wf_typ_eq_sub {P : PtsSig} : forall {Δ : ctx P} {A A'},
+    {{ Δ ⊢ A ≈ A' }} ->
+    forall Γ σ,
+    {{ Γ ⊢s σ : Δ }} ->
+    {{ Γ ⊢ A[σ] ≈ A'[σ] }}.
+Proof. mauto. Qed.
+
+#[export]
+Hint Resolve wf_typ_eq_sub : mcpts.
+
+Lemma wf_subtyp_univ_weaken {P : PtsSig} : forall {Γ : ctx P} {s1 s2 A},
+    {{ Γ ⊢ Sort@s1 ≈ Sort@s1 }} ->
+    {{ ⊢ Γ, A::Sort@s2 }} ->
+    {{ Γ, A::Sort@s2 ⊢ Sort@s1 ≈ Sort@s1 }}.
+Proof. mauto. Qed.
+
+Lemma var_compose_subs {P : PtsSig} : forall {Γ : ctx P} {τ Δ σ Ψ s A x},
+    {{ Ψ ⊢ A : Sort@s }} ->
+    {{ Δ ⊢s σ : Ψ }} ->
+    {{ Γ ⊢s τ : Δ }} ->
+    {{ #x : A[σ][τ] :: Sort@s ∈ Γ }} ->
+    {{ Γ ⊢ #x : A[σ∘τ] }}.
+Proof.
+  intros.
+  eapply wf_conv; mauto 3.
+  econstructor; mauto.
+Qed.
+
+#[export]
+Hint Resolve var_compose_subs : mcpts.
+
+Lemma sub_lookup_var0 {P : PtsSig} : forall (Δ : ctx P) Γ σ M1 M2 B s,
+    {{ Δ ⊢s σ : Γ }} ->
+    {{ Γ ⊢ B : Sort@s }} ->
+    {{ Δ ⊢ M1 : B[σ] }} ->
+    {{ Δ ⊢ M2 : B[σ] }} ->
+    {{ Δ ⊢ #0[σ,,M1,,M2] ≈ M2 : B[σ] }}.
+Proof.
+  intros.
+  assert {{ Γ, B::Sort@s ⊢ B[Wk] : Sort@s }} by mauto.
+  assert {{ Δ ⊢s σ,,M1 : Γ, B::Sort@s }} by mauto 4.
+  assert {{ Δ ⊢ B[Wk][σ,,M1] : Sort@s }} by mauto 4.
+  assert {{ Δ ⊢ B[Wk][σ,,M1] ≈ B[σ] }}.
+  {
+    transitivity {{{ B[Wk∘(σ,,M1)] }}}.
+    - eapply exp_eq_sub_compose_typ; mauto 4.
+    - eapply exp_eq_sub_cong_typ2'; mauto 4.
+  }
+  eapply wf_exp_eq_conv;
+    [eapply wf_exp_eq_var_0_sub with (A := {{{ B[Wk] }}}) | |];
+    mauto 4.
+Qed.
+
+Lemma id_sub_lookup_var0 {P : PtsSig} : forall (Γ : ctx P) M1 M2 B s,
+    {{ Γ ⊢ B : Sort@s }} ->
+    {{ Γ ⊢ M1 : B }} ->
+    {{ Γ ⊢ M2 : B }} ->
+    {{ Γ ⊢ #0[Id,,M1,,M2] ≈ M2 : B }}.
+Proof.
+  intros.
+  eapply wf_exp_eq_conv;
+    [eapply sub_lookup_var0 | |];
+    mauto 3.
+Qed.
+
+Lemma sub_lookup_var1 {P : PtsSig} : forall (Δ : ctx P) Γ σ M1 M2 B s,
+    {{ Δ ⊢s σ : Γ }} ->
+    {{ Γ ⊢ B : Sort@s }} ->
+    {{ Δ ⊢ M1 : B[σ] }} ->
+    {{ Δ ⊢ M2 : B[σ] }} ->
+    {{ Δ ⊢ #1[σ,,M1,,M2] ≈ M1 : B[σ] }}.
+Proof.
+  intros.
+  assert {{ Γ, B::Sort@s ⊢ B[Wk] : Sort@s }} by mauto.
+  assert {{ Δ ⊢s σ,,M1 : Γ, B::Sort@s }} by mauto 4.
+  assert {{ Δ ⊢ B[Wk][σ,,M1] : Sort@s }} by mauto 4.
+  assert {{ Δ ⊢ B[Wk][σ,,M1] ≈ B[σ] }}.
+  {
+    transitivity {{{ B[Wk∘(σ,,M1)] }}}.
+    - eapply exp_eq_sub_compose_typ; mauto 4.
+    - eapply exp_eq_sub_cong_typ2'; mauto 4.
+  }
+  transitivity {{{ #0[σ,,M1] }}}.
+  - eapply wf_exp_eq_conv;
+      [eapply wf_exp_eq_var_S_sub | |];
+      mauto 4.
+  - eapply wf_exp_eq_conv;
+    [eapply wf_exp_eq_var_0_sub with (A := B) | |];
+    mauto.
+Qed.
+
+Lemma id_sub_lookup_var1 {P : PtsSig} : forall (Γ : ctx P) M1 M2 B s,
+    {{ Γ ⊢ B : Sort@s }} ->
+    {{ Γ ⊢ M1 : B }} ->
+    {{ Γ ⊢ M2 : B }} ->
+    {{ Γ ⊢ #1[Id,,M1,,M2] ≈ M1 : B }}.
+Proof.
+  intros.
+  eapply wf_exp_eq_conv;
+    [eapply sub_lookup_var1 | |];
+    mauto 3.
+Qed.
+
+Lemma exp_eq_var_1_sub_q_sigma {P : PtsSig} : forall {Γ : ctx P} {A s1 B s2 σ Δ},
+    {{ Δ ⊢ B : Sort@s1 }} ->
+    {{ Δ, B::Sort@s1 ⊢ A : Sort@s2 }} ->
+    {{ Γ ⊢s σ : Δ }} ->
+    {{ Γ, B[σ]::Sort@s1, A[q σ]::Sort@s2 ⊢ #1[q (q σ)] ≈ #1 : B[σ][Wk∘Wk] }}.
+Proof with mautosolve 4.
+  intros.
+  assert {{ ⊢ Δ }} by mauto 2.
+  assert {{ Γ, B[σ]::Sort@s1 ⊢s q σ : Δ, B::Sort@s1 }} by mauto 2.
+  assert {{ ⊢ Γ, B[σ]::Sort@s1 }} by mauto 3.
+  assert {{ ⊢ Γ, B[σ]::Sort@s1, A[q σ]::Sort@s2 }} by mauto 3.
+  assert {{ Δ, B::Sort@s1 ⊢ B[Wk] : Sort@s1 }} by mauto 4.
+  assert {{ Δ, B::Sort@s1 ⊢ #0 : B[Wk] }} by mauto 3.
+  assert {{ Γ, B[σ]::Sort@s1, A[q σ]::Sort@s2 ⊢ #0 : A[q σ][Wk] }} by mauto 2.
+  assert {{ Γ, B[σ]::Sort@s1, A[q σ]::Sort@s2 ⊢ A[q σ∘Wk] ≈ A[q σ][Wk] : Sort@s2 }} by (eapply wf_exp_eq_conv; mauto 4).
+  assert {{ Γ, B[σ]::Sort@s1, A[q σ]::Sort@s2 ⊢s q σ∘Wk : Δ, B::Sort@s1 }} by mauto 3.
+  assert {{ Γ, B[σ]::Sort@s1, A[q σ]::Sort@s2 ⊢ #0 : A[q σ∘Wk] }} by mauto 3.
+  assert {{ Γ ⊢ B[σ] : Sort@s1 }} by mauto 2.
+  assert {{ Γ, B[σ]::Sort@s1 ⊢s Wk : Γ }} by mauto 2.
+  assert {{ Γ, B[σ]::Sort@s1, A[q σ]::Sort@s2 ⊢s Wk : Γ, B[σ]::Sort@s1 }} by mauto 2.
+  assert {{ Γ, B[σ]::Sort@s1 ⊢ B[σ][Wk] : Sort@s1 }} by mauto 2.
+  assert {{ Γ, B[σ]::Sort@s1, A[q σ]::Sort@s2 ⊢ B[σ][Wk][Wk] : Sort@s1 }} by mauto 2.
+  assert {{ Γ, B[σ]::Sort@s1 ⊢ B[Wk][q σ] ≈ B[σ][Wk] }} by (eapply exp_eq_sub_sub_compose_cong_typ; mauto 3).  
+  assert {{ Γ, B[σ]::Sort@s1 ,A[q σ]::Sort@s2 ⊢ B[Wk][q σ∘Wk] ≈ B[σ][Wk][Wk] }} by (transitivity {{{ B[Wk][q σ][Wk] }}}; mauto 3).
+  assert {{ Γ, B[σ]::Sort@s1, A[q σ]::Sort@s2 ⊢ #1[q (q σ)] ≈ #0[q σ∘Wk] : B[σ][Wk][Wk] }} by mauto 4.
+  assert {{ Γ, B[σ]::Sort@s1, A[q σ]::Sort@s2 ⊢ #0[q σ∘Wk] ≈ #0[q σ][Wk] : B[σ][Wk][Wk] }} by mauto 4. 
+  assert {{ Γ, B[σ]::Sort@s1 ⊢s σ∘Wk : Δ }} by mauto 2.
+  assert {{ Γ, B[σ]::Sort@s1 ⊢ #0 : B[σ∘Wk] }} by mauto 2.
+  assert {{ Γ, B[σ]::Sort@s1 ⊢ #0[q σ] ≈ #0 : B[σ∘Wk] }} by mauto 2.
+  assert {{ Γ, B[σ]::Sort@s1, A[q σ]::Sort@s2 ⊢ #0[q σ][Wk] ≈ #0[Wk] : B[σ∘Wk][Wk] }} by mauto 3.
+  assert {{ Γ, B[σ]::Sort@s1, A[q σ]::Sort@s2 ⊢ B[σ∘Wk][Wk] ≈ B[σ][Wk][Wk] }} by mauto 4.
+  assert {{ Γ, B[σ]::Sort@s1, A[q σ]::Sort@s2 ⊢ #0[q σ][Wk] ≈ #0[Wk] : B[σ][Wk][Wk] }} by mauto 3.
+  assert {{ Γ, B[σ]::Sort@s1, A[q σ]::Sort@s2 ⊢ #1[q (q σ)] ≈ #1 : B[σ][Wk][Wk] }} by (do 2 etransitivity; mauto 2).
+  assert {{ Γ, B[σ]::Sort@s1, A[q σ]::Sort@s2 ⊢s Wk∘Wk : Γ }} by mauto 2.
+  assert {{ Γ, B[σ]::Sort@s1, A[q σ]::Sort@s2 ⊢ B[σ][Wk∘Wk] : Sort@s1 }} by mauto 2.
+  eapply wf_exp_eq_conv; mauto 3.
+Qed.
+
+(** *** Type Presuppositions *)
+
+Lemma presup_exp_typ {P : PtsSig} : forall {Γ : ctx P} {M A},
+    {{ Γ ⊢ M : A }} ->
+    {{ Γ ⊢ A }}.
+Proof.
+  induction 1; assert {{ ⊢ Γ }} by mauto 3; destruct_conjs; mauto 3.
+
+  - enough {{ Γ ⊢s Id,,N : Γ, A::Sort@s1 }}; mauto 3.
+  - assert ({{ Γ ⊢ A : Sort@s }} /\ exists s', {{{ Sort@s }}} = {{{ Sort@s' }}}) by mauto 2.
+    destruct_conjs; mauto.
+Qed.
+
+Lemma presup_exp {P : PtsSig} : forall {Γ : ctx P} {M A},
+    {{ Γ ⊢ M : A }} ->
+    {{ ⊢ Γ }} /\ {{ Γ ⊢ A }}.
+Proof.
+  mauto 4 using presup_exp_typ.
+Qed.
+
+Lemma presup_typ {P : PtsSig} : forall {Γ : ctx P} {A},
+    {{ Γ ⊢ A }} ->
+    {{ ⊢ Γ }}.
+Proof.
+  intros *.
+  inversion_clear 1; mauto.
+Qed.
+
+
+(** *** Consistency Helper *)
+
+Lemma no_closed_neutral {P : PtsSig} : forall {A : exp P} {W : ne P},
+    ~ {{ ⋅ ⊢ W : A }}.
+Proof.
+  intros * H.
+  dependent induction H; destruct W;
+    try (simpl in *; congruence);
+    autoinjections;
+    intuition.
+  inversion_by_head (@ctx_lookup P).
+Qed.
+#[export]
+Hint Resolve no_closed_neutral : mcpts.
+
+
+
+
+
+
+
+
+
+
+
+
+
+
+
+
+(*
+
+(** ** Basic Context Properties *)
+
 Lemma ctx_lookup_lt {P : PtsSig} : forall {Γ : Ctx P} {A x s},
     {{ #x : A :: Sort@s ∈ Γ }} ->
     x < length Γ.
@@ -1153,3 +2140,6 @@ Proof.
 Qed.
 #[export]
 Hint Resolve no_closed_neutral : mcpts.
+
+
+*)
