mechanization/theories/Core/Syntactic/SystemOpt.v
@@ -5,20 +5,19 @@ From McPTS.Core.Syntactic Require Export CoreInversions Presup.
 Import Syntax_Notations.
 
 
+ 
 Add Parametric Morphism {P : PtsSig} (s : St P) Γ : (wf_exp Γ)
-    with signature eq_exp Γ {{{ Sort@s }}} ==> eq ==> iff as wf_exp_morphism_iff3.
+    with signature wf_exp_eq Γ {{{ Sort@s }}} ==> eq ==> iff as wf_exp_morphism_iff3.
 Proof with mautosolve.
   split; intros; gen_presups;
-    eapply wf_exp_conv; mauto 2.
-  econstructor; mauto 2.
+    eapply wf_exp_conv; mauto 3.
 Qed.
 
-Add Parametric Morphism {P : PtsSig} (s : St P) Γ : (eq_exp Γ)
-    with signature eq_exp Γ {{{ Sort@s }}} ==> eq ==> eq ==> iff as wf_exp_eq_morphism_iff3.
+Add Parametric Morphism {P : PtsSig} (s : St P) Γ : (wf_exp_eq Γ)
+    with signature wf_exp_eq Γ {{{ Sort@s }}} ==> eq ==> eq ==> iff as wf_exp_eq_morphism_iff3.
 Proof with mautosolve.
   split; intros; gen_presups;
-    eapply eq_exp_conv; mauto 2.
-  econstructor; mauto 2.
+    eapply wf_exp_eq_conv; mauto 3.
 Qed.
 
 #[local]
@@ -27,14 +26,12 @@ Ltac impl_opt_constructor :=
   gen_presups;
   mautosolve 4.
 
-Corollary wf_conv' {P : PtsSig} : forall (Γ : Ctx P) M A A',
+Corollary wf_conv' {P : PtsSig} : forall (Γ : ctx P) M A A',
     {{ Γ ⊢ M : A }} ->
     {{ Γ ⊢ A ≈ A' }} ->
     {{ Γ ⊢ M : A' }}.
 Proof.
-  intros;
-  gen_presups;
-  eapply wf_exp_conv; mauto 2.
+  impl_opt_constructor.
 Qed.
 
 #[export]
@@ -42,13 +39,12 @@ Hint Resolve wf_conv' : mcpts.
 #[export]
 Remove Hints wf_conv : mcpts.
 
-Corollary wf_exp_eq_conv' {P : PtsSig} : forall (Γ : Ctx P) M M' A A' s,
+Corollary wf_exp_eq_conv' {P : PtsSig} : forall (Γ : ctx P) M M' A A',
    {{ Γ ⊢ M ≈ M' : A }} ->
-   {{ Γ ⊢ A ≈ A' : Sort@s }} ->
+   {{ Γ ⊢ A ≈ A' }} ->
    {{ Γ ⊢ M ≈ M' : A' }}.
 Proof.
-  intros.
-  eapply eq_exp_conv; mauto 2.
+  impl_opt_constructor.
 Qed.
 
 #[export]
@@ -57,7 +53,7 @@ Hint Resolve wf_exp_eq_conv' : mcpts.
 Remove Hints wf_exp_eq_conv : mcpts.
 
 
-Corollary wf_ctx_eq_extend' {P : PtsSig} : forall {Γ : Ctx P} {Δ A A' s},
+Corollary wf_ctx_eq_extend' {P : PtsSig} : forall {Γ : ctx P} {Δ A A' s},
     {{ ⊢ Γ ≈ Δ }} ->
     {{ Γ ⊢ A ≈ A' : Sort@s }} ->
     {{ ⊢ Γ, A::Sort@s ≈ Δ, A'::Sort@s }}.
@@ -71,40 +67,37 @@ Qed.
 #[export]
 Hint Resolve wf_ctx_eq_extend' : mcpts.
 #[export]
-Remove Hints eq_ctx_cons : mcpts.
+Remove Hints wf_ctx_eq_extend : mcpts.
 
 
-Corollary wf_pi_max {P : PtsSig} : forall {Γ : Ctx P} {A B s1 s2 s3} {r : Ru P s1 s2 s3},
+Corollary wf_pi {P : PtsSig} : forall {Γ : ctx P} {A B s1 s2 s3} {r : Ru P s1 s2 s3},
     {{ Γ ⊢ A : Sort@s1 }} ->
     {{ Γ, A::Sort@s1 ⊢ B : Sort@s2 }} ->
     {{ Γ ⊢ Π r A B : Sort@s3 }}.
 Proof.
-  intros.
-  econstructor; mauto 2.
+  intros; mauto 2.
 Qed.
 
 #[export]
-Hint Resolve wf_pi_max : mcpts.
+Hint Resolve wf_pi : mcpts.
 
-Corollary wf_fn' {P : PtsSig} : forall {Γ : Ctx P} {A M B s1 s2 s3} {r : Ru P s1 s2 s3},
+Corollary wf_fn' {P : PtsSig} : forall {Γ : ctx P} {A M B s1 s2 s3} {r : Ru P s1 s2 s3},
     {{ Γ, A::Sort@s1 ⊢ M : B }} ->
     {{ Γ, A::Sort@s1 ⊢ B : Sort@s2 }} ->
     {{ Γ ⊢ λ r A M : Π r A B }}.
 Proof.
-  intros.
-  gen_presups.
-  econstructor; mauto 2.
+  impl_opt_constructor.
 Qed.
 
 #[export]
 Hint Resolve wf_fn' : mcpts.
 #[export]
-Remove Hints wf_exp_lam : mcpts.
+Remove Hints wf_fn : mcpts.
 
-Corollary wf_app' {P : PtsSig} : forall {Γ : Ctx P} {M N A B s1 s2 s3} {r : Ru P s1 s2 s3},
+Corollary wf_app' {P : PtsSig} : forall {Γ : ctx P} {M N A B s1 s2 s3} {r : Ru P s1 s2 s3},
     {{ Γ ⊢ M : Π r A B }} ->
     {{ Γ ⊢ N : A }} ->
-    {{ Γ ⊢ M N : [Id,,N]B }}.
+    {{ Γ ⊢ M N : B[Id,,N] }}.
 Proof.
   intros.
   gen_presups.
@@ -120,12 +113,12 @@ Qed.
 #[export]
 Hint Resolve wf_app' : mcpts.
 #[export]
-Remove Hints wf_exp_app : mcpts.
+Remove Hints wf_app : mcpts.
 
-Lemma wf_exp_eq_typ_sub' {P : PtsSig} : forall (Γ : Ctx P) σ Δ s1 s2,
-    {{ Γ ⊢s σ : Δ }} ->
+Lemma wf_exp_eq_typ_sub' {P : PtsSig} : forall (Γ : ctx P) σ Δ s1 s2,
     Ax P s1 s2 ->
-    {{ Γ ⊢ [σ]Sort@s1 ≈ Sort@s1 : Sort@s2 }}.
+    {{ Γ ⊢s σ : Δ }} ->
+    {{ Γ ⊢ Sort@s1[σ]≈ Sort@s1 : Sort@s2 }}.
 Proof.
   intros.
   econstructor; mauto 2.
@@ -138,51 +131,7 @@ Hint Resolve wf_exp_eq_typ_sub' : mcpts.
 Hint Rewrite -> @wf_exp_eq_typ_sub' using solve [lia | mauto 3] : mcpts.
 
 
-(* These results don't really make sense in our setting *)
-
-(* Corollary wf_exp_eq_pi_sub_max : forall {Γ σ Δ A i B j}, *)
-(*     {{ Γ ⊢s σ : Δ }} -> *)
-(*     {{ Δ ⊢ A : Type@i }} -> *)
-(*     {{ Δ, A ⊢ B : Type@j }} -> *)
-(*     {{ Γ ⊢ (Π A B)[σ] ≈ Π (A[σ]) (B[q σ]) : Type@(max i j) }}. *)
-(* Proof. *)
-(*   intros. *)
-(*   assert {{ Δ ⊢ A : Type@(max i j) }} by mauto using lift_exp_max_left. *)
-(*   assert {{ Δ, A ⊢ B : Type@(max i j) }} by mauto using lift_exp_max_right. *)
-(*   mauto. *)
-(* Qed. *)
-
-(* #[export] *)
-(* Hint Resolve wf_exp_eq_pi_sub_max : mcpts. *)
-
-(* Corollary wf_exp_eq_pi_cong' : forall {Γ A A' B B' i}, *)
-(*     {{ Γ ⊢ A ≈ A' : Type@i }} -> *)
-(*     {{ Γ, A ⊢ B ≈ B' : Type@i }} -> *)
-(*     {{ Γ ⊢ Π A B ≈ Π A' B' : Type@i }}. *)
-(* Proof. *)
-(*   impl_opt_constructor. *)
-(* Qed. *)
-
-(* #[export] *)
-(* Hint Resolve wf_exp_eq_pi_cong' : mcpts. *)
-(* #[export] *)
-(* Remove Hints wf_exp_eq_pi_cong : mcpts. *)
-
-(* Corollary wf_exp_eq_pi_cong_max : forall {Γ A A' i B B' j}, *)
-(*     {{ Γ ⊢ A ≈ A' : Type@i }} -> *)
-(*     {{ Γ, A ⊢ B ≈ B' : Type@j }} -> *)
-(*     {{ Γ ⊢ Π A B ≈ Π A' B' : Type@(max i j) }}. *)
-(* Proof. *)
-(*   intros. *)
-(*   assert {{ Γ ⊢ A ≈ A' : Type@(max i j) }} by eauto using lift_exp_eq_max_left. *)
-(*   assert {{ Γ, A ⊢ B ≈ B' : Type@(max i j) }} by eauto using lift_exp_eq_max_right. *)
-(*   mauto. *)
-(* Qed. *)
-
-(* #[export] *)
-(* Hint Resolve wf_exp_eq_pi_cong_max : mcpts. *)
-
-Corollary wf_exp_eq_fn_cong' {P : PtsSig} : forall {Γ : Ctx P} {A A' s1 s2 s3 B M M'} {r : Ru P s1 s2 s3},
+Corollary wf_exp_eq_fn_cong' {P : PtsSig} : forall {Γ : ctx P} {A A' s1 s2 s3 B M M'} {r : Ru P s1 s2 s3},
     {{ Γ ⊢ A ≈ A' : Sort@s1 }} ->
     {{ Γ, A::Sort@s1 ⊢ M ≈ M' : B }} ->
     {{ Γ, A::Sort@s1 ⊢ B :Sort@s2 }} ->
@@ -198,78 +147,78 @@ Qed.
 #[export]
 Hint Resolve wf_exp_eq_fn_cong' : mcpts.
 #[export]
-Remove Hints eq_exp_cong_lam : mcpts.
+Remove Hints wf_exp_eq_fn_cong : mcpts.
 
-Corollary wf_exp_eq_fn_sub' {P : PtsSig} : forall {Γ : Ctx P} {σ Δ A M B s1 s2 s3} {r : Ru P s1 s2 s3},
+Corollary wf_exp_eq_fn_sub' {P : PtsSig} : forall {Γ : ctx P} {σ Δ A M B s1 s2 s3} {r : Ru P s1 s2 s3},
     {{ Γ ⊢s σ : Δ }} ->
     {{ Δ, A::Sort@s1 ⊢ M : B }} ->
     {{ Δ, A::Sort@s1 ⊢ B : Sort@s2 }} ->
-    {{ Γ ⊢ [σ](λ r A M) ≈ λ r [σ]A [(Wk∘σ),,#0]M : [σ](Π r A B) }}.
+    {{ Γ ⊢ (λ r A M)[σ] ≈ λ r A[σ] M[q σ] : (Π r A B)[σ] }}.
 Proof.
-  intros.
-  gen_presups.
-  econstructor; mauto 2.
-  econstructor; mauto 2.
+  impl_opt_constructor.
 Qed.
 
 #[export]
 Hint Resolve wf_exp_eq_fn_sub' : mcpts.
 #[export]
-Remove Hints eq_exp_prop_lam : mcpts.
+Remove Hints wf_exp_eq_fn_sub : mcpts.
 
-Corollary wf_exp_eq_app_cong' {P : PtsSig} : forall {Γ : Ctx P} {A B M M' N N' s1 s2 s3} {r : Ru P s1 s2 s3},
+Corollary wf_exp_eq_app_cong' {P : PtsSig} : forall {Γ : ctx P} {A B M M' N N' s1 s2 s3} {r : Ru P s1 s2 s3},
     {{ Γ ⊢ M ≈ M' : Π r A B }} ->
     {{ Γ ⊢ N ≈ N' : A }} ->
-    {{ Γ ⊢ M N ≈ M' N' : [Id,,N]B }}.
+    {{ Γ ⊢ M N ≈ M' N' : B[Id,,N] }}.
 Proof.
   intros.
+  gen_presups.
+  assert ({{ Γ ⊢ A : Sort@s1 }} /\ {{ Γ, A::Sort@s1 ⊢ B : Sort@s2 }}) by mauto 2.
+  destruct_conjs.
   econstructor; mauto 2.
-  assert {{ Γ ⊢ Π r A B }} by (eapply presup_exp_eq; mauto 2).
-  eapply wf_typ_pi_inversion; mauto 2.
 Qed.  
 
 #[export]
 Hint Resolve wf_exp_eq_app_cong' : mcpts.
 #[export]
-Remove Hints eq_exp_cong_app : mcpts.
+Remove Hints wf_exp_eq_app_cong : mcpts.
 
-Corollary wf_exp_eq_app_sub' {P : PtsSig} : forall {Γ : Ctx P} {σ Δ A B M N s1 s2 s3} {r : Ru P s1 s2 s3},
+Corollary wf_exp_eq_app_sub' {P : PtsSig} : forall {Γ : ctx P} {σ Δ A B M N s1 s2 s3} {r : Ru P s1 s2 s3},
     {{ Γ ⊢s σ : Δ }} ->
     {{ Δ ⊢ M : Π r A B }} ->
     {{ Δ ⊢ N : A }} ->
-    {{ Γ ⊢ [σ](M N) ≈ [σ]M [σ]N : [σ,,[σ]N]B }}.
+    {{ Γ ⊢ (M N)[σ] ≈ M[σ] N[σ] : B[σ,,N[σ]] }}.
 Proof.
   intros.
   gen_presups.
-  econstructor; mauto 2.
+  assert ({{ Δ ⊢ A : Sort@s1 }} /\ {{ Δ, A::Sort@s1 ⊢ B : Sort@s2 }}) by mauto 2.
+  destruct_conjs.
+  econstructor; mauto.
 Qed.
 
 #[export]
 Hint Resolve wf_exp_eq_app_sub' : mcpts.
 #[export]
-Remove Hints eq_exp_prop_app : mcpts.
+Remove Hints wf_exp_eq_app_sub : mcpts.
 
-Corollary wf_exp_eq_pi_beta' {P : PtsSig} : forall {Γ : Ctx P} {A B M N s1 s2 s3} {r : Ru P s1 s2 s3},
+Corollary wf_exp_eq_pi_beta' {P : PtsSig} : forall {Γ : ctx P} {A B M N s1 s2 s3} {r : Ru P s1 s2 s3},
     {{ Γ, A::Sort@s1 ⊢ M : B }} ->
     {{ Γ, A::Sort@s1 ⊢ B : Sort@s2 }} ->
     {{ Γ ⊢ N : A }} ->
-    {{ Γ ⊢ (λ r A M) N ≈ [Id,,N]M : [Id,,N]B }}.
+    {{ Γ ⊢ (λ r A M) N ≈ M[Id,,N] : B[Id,,N] }}.
 Proof.
-  intros.
-  gen_presups.
-  econstructor; mauto 2.
+  impl_opt_constructor.
 Qed.
 
 #[export]
 Hint Resolve wf_exp_eq_pi_beta' : mcpts.
 #[export]
-Remove Hints eq_exp_beta : mcpts.
+Remove Hints wf_exp_eq_pi_beta : mcpts.
 
-Corollary wf_exp_eq_pi_eta' {P : PtsSig} : forall {Γ : Ctx P} {A B M s1 s2 s3} {r : Ru P s1 s2 s3},
+Corollary wf_exp_eq_pi_eta' {P : PtsSig} : forall {Γ : ctx P} {A B M s1 s2 s3} {r : Ru P s1 s2 s3},
     {{ Γ ⊢ M : Π r A B }} ->
-    {{ Γ ⊢ M ≈ λ r A ([Wk]M #0) : Π r A B }}.
+    {{ Γ ⊢ M ≈ λ r A (M[Wk] #0) : Π r A B }}.
 Proof.
   intros.
   gen_presups.
+  assert ({{ Γ ⊢ A : Sort@s1 }} /\ {{ Γ, A::Sort@s1 ⊢ B : Sort@s2 }}) by mauto 2.
+  destruct_conjs.  
   econstructor; mauto 2.
 Qed.
